Verbatim/memo/impl.v
@@ -7,6 +7,7 @@ Require Import Coq.Numbers.NatInt.NZOrder.
 From Verbatim Require Import ltac.
 From Verbatim Require Import memo.
 From Verbatim Require Import lexer.impl.
+From Verbatim Require Import lexer.lemmas.
 
 Module ImplFn (Import MEM : memo.T).
 
@@ -16,6 +17,7 @@ Module ImplFn (Import MEM : memo.T).
   Import Defs.NaiveLexer.MPref.
   Import MEM.STT.Defs.
   Import MEM.STT.Ty.
+  Module Import L := LemmasFn MEM.STT.
 
   Module Export Utils.
 
@@ -72,58 +74,60 @@ Module ImplFn (Import MEM : memo.T).
   Module Export MPref.
          
     (** Single-rule Prefixer **)
-    Fixpoint max_pref_fn__M (M : Memo) (s : String) (state : State)
-    : Memo * option (String * String) :=
+    Fixpoint max_pref_fn__M (M : Memo) (s : String) (i : index) (state : State) 
+    : Memo * option (String * String * index) :=
       match s with
       (* in a regex approach, accepting := nullable *)
-      | [] => if accepting state then (M, Some ([],[])) else (M, None)
+      | [] => if accepting state then (M, Some ([],[],i))
+             else ((set_Memo M (fst state) i None), None)
       | a :: s' =>
         let
           (* in a regex approach, transition := derivative *)
           state' := transition a state in
         let
-          lookup := get_Memo M (fst state') s' in
+          lookup := get_Memo M (fst state') (decr i) in
         let
           mpxs :=
           match lookup with
-          | None => max_pref_fn__M M s' state'
+          | None => max_pref_fn__M M s' (decr i) state' 
           | Some o => (M, o)
           end
         in
 
         match mpxs with
-        | (M', None) => if (accepting state') then (M' , Some ([a], s')) else
-                         if (accepting state) then (M', Some ([], s)) else
-                           ((set_Memo M' (fst state) s None), None)
-        | (M', Some (p, q)) => (M', Some (a :: p, q))
+        | (M', None) => if (accepting state') then (M' , Some ([a], s', (decr i))) else
+                         if (accepting state) then (M', Some ([], s, i)) else
+                           ((set_Memo M' (fst state) i None), None)
+        | (M', Some (p, q, qi)) => (M', Some (a :: p, q, qi))
         end
       end.
 
     (** Multi-rule Prefixer **)
-    Definition extract_fsm_for_max__M (code : String) (sru : Memo * (Label * State))
-      : Memo * (Label * option (Prefix * Suffix)) :=
+    Definition extract_fsm_for_max__M (code : String) (i : index)
+               (sru : Memo * (Label * State)) 
+      : Memo * (Label * option (Prefix * Suffix * index)) :=
       match sru with
         (M, (a, fsm)) =>
-        match max_pref_fn__M M code fsm with
+        match max_pref_fn__M M code i fsm with
           (M', o) => (M', (a, o))
         end
       end.
 
-
-    Definition max_prefs__M (Ms : list Memo) (code : String) (erules : list (Label * State))
-      : (list Memo) * list (Label * option (Prefix * Suffix))
+    Definition max_prefs__M (Ms : list Memo) (code : String) 
+               (i : index) (erules : list (Label * State))
+      : (list Memo) * list (Label * option (Prefix * Suffix * index))
       :=
         let
           zipped := zip Ms erules
         in
         let
-          mapped := map (extract_fsm_for_max__M code) zipped
+          mapped := map (extract_fsm_for_max__M code i) zipped
         in
         unzip mapped.
 
     Fixpoint max_of_prefs__M (mprefs : list Memo
-                                     * list (Label * (option (Prefix * Suffix))))
-      : list Memo * Label * option (Prefix * Suffix) :=
+                                     * list (Label * (option (Prefix * Suffix * index))))
+      : list Memo * Label * option (Prefix * Suffix * index) :=
       match mprefs with
         (Ms, prefs) =>
         match max_of_prefs prefs with
@@ -137,51 +141,62 @@ Module ImplFn (Import MEM : memo.T).
 
     Module Export MemoEq.
 
-      Lemma lexy_correct : forall M pnt z o d,
-        lexy M d
-        -> get_Memo M pnt z = Some (o)
-        -> max_pref_fn z (pnt, d) = o.
+
+      Lemma ith_suffix_cons : forall z code a i, 
+        ith_suffix code (a :: z) i -> ith_suffix code z (decr i).
+      Admitted.
+      
+      Lemma lexy_correct : forall M pnt z o d code i,
+        lexy code M d
+        -> ith_suffix code z i
+        -> get_Memo M pnt i = Some (o)
+        -> max_pref_fn z i (pnt, d) = o.
       Proof.
-        intros. unfold lexy in H. apply H in H0. auto.
+        intros. unfold lexy in H. eapply H in H0; eauto.
       Qed.
 
-      Theorem mpref_memo_eq_lexy_F : forall z pnt o M M' d,
-          lexy M d
-          -> max_pref_fn__M M z (pnt, d) = (M', o)
-          -> max_pref_fn z (pnt, d) = o.
+      Theorem mpref_memo_eq_lexy_F : forall z pnt o M M' d code i,
+          lexy code M d
+          -> ith_suffix code z i
+          -> max_pref_fn__M M z i (pnt, d) = (M', o)
+          -> max_pref_fn z i (pnt, d) = o.
       Proof.
         induction z; intros.
         - simpl in *. repeat dm; repeat inj_all; auto.
         - simpl in *.
           repeat dm;
-            try(eapply lexy_correct in H; eauto; unfold fst in H; dm; apply transition_Delta in E5;
-                repeat inj_all; rewrite H in *; repeat inj_all; auto; try discriminate);
-            try(eapply lexy_correct in H; eauto; unfold fst in H; dm; apply transition_Delta in E6;
-                repeat inj_all; rewrite H in *; repeat inj_all; auto; try discriminate);
-            try (destruct (transition a (pnt, d)) eqn:H1; apply transition_Delta in H1;
-                 repeat inj_all; apply IHz in E; auto; rewrite E in *;
-                 repeat inj_all; auto; discriminate).
-          repeat inj_all. auto.
+          try( repeat inj_all; unfold lexy in H; apply ith_suffix_cons in H0;
+            eapply H in E3; eauto; unfold fst in E3; dm; apply transition_Delta in E; subst;
+            rewrite E3 in *; repeat inj_all; auto; discriminate );
+          try( repeat inj_all; apply ith_suffix_cons in H0;
+               destruct (transition a (pnt, d)) eqn:E7; apply transition_Delta in E7;
+               rewrite E7 in *; eapply IHz in E; eauto; rewrite E in *; repeat inj_all;
+               auto; discriminate ).
+          + repeat inj_all. unfold lexy in H. apply ith_suffix_cons in H0. eapply H in E2; eauto.
+            unfold fst in E2. dm. apply transition_Delta in E. rewrite E in *. rewrite E2 in *.
+            discriminate.
+          + repeat inj_all. unfold lexy in H. apply ith_suffix_cons in H0. eapply H in E2; eauto.
       Qed.
       
-      Lemma cons_mprefs__M : forall m Ms z a rules m' Ms' p lst,
-          max_prefs__M (m :: Ms) z (a :: rules) = (m' :: Ms', p :: lst)
-          -> max_prefs__M [m] z [a] = ([m'], [p]) /\ max_prefs__M Ms z rules = (Ms', lst).
+      Lemma cons_mprefs__M : forall m Ms z a rules m' Ms' p lst i,
+          max_prefs__M (m :: Ms) z i (a :: rules) = (m' :: Ms', p :: lst)
+          -> max_prefs__M [m] z i [a] = ([m'], [p]) /\ max_prefs__M Ms z i rules = (Ms', lst).
       Proof.
         intros. unfold max_prefs__M in *. simpl in *. repeat dm; repeat inj_all; subst. auto.
       Qed.
 
-      Theorem mprefs_memo_F : forall z rules Ms Ms' lst,
-          lexy_list (zip Ms (map ssnd rules))
+      Theorem mprefs_memo_F : forall z rules Ms Ms' lst i code,
+          lexy_list code (zip Ms (map ssnd rules))
           -> length Ms = length rules
-          -> max_prefs__M Ms z rules = (Ms', lst)
-          -> max_prefs z rules = lst.
+          -> max_prefs__M Ms z i rules = (Ms', lst)
+          -> ith_suffix code z i
+          -> max_prefs z i rules = lst.
       Proof.
         induction rules; intros.
         - destruct Ms;
-            unfold max_prefs__M in H1; simpl in H1; repeat inj_all; subst; auto; discriminate.
+            unfold max_prefs__M in H1; simpl in H1; repeat inj_all; subst; auto.
         - destruct Ms; try(discriminate).
-          assert(A0 : lexy_list (zip Ms (map ssnd rules))).
+          assert(A0 : lexy_list code (zip Ms (map ssnd rules))).
           { unfold lexy_list in *. intros. apply H. simpl. right. auto. }
           assert(A1 : length Ms = length rules).
           { simpl in H0. inv H0. auto. }
@@ -193,7 +208,7 @@ Module ImplFn (Import MEM : memo.T).
               apply cons_mprefs__M in H1. eapply IHrules in A0; destruct H1; eauto.
               unfold max_prefs__M in e. simpl in e. repeat dm. repeat inj_all; subst.
               destruct p0.
-              assert(A2 : lexy m d).
+              assert(A2 : lexy code m d).
               { unfold lexy_list in *. apply H. simpl. left. auto. }
               eapply mpref_memo_eq_lexy_F in A2; eauto. subst. auto.
       Qed.
@@ -202,13 +217,15 @@ Module ImplFn (Import MEM : memo.T).
 
     Module Export Accessible.
       
-      Lemma acc_helper__M : forall Ms code rules Ms' label o,
-        lexy_list (zip Ms (map ssnd rules))
+      Lemma acc_helper__M : forall Ms code rules Ms' label o i orig,
+        lexy_list orig (zip Ms (map ssnd rules))
         -> length Ms = length rules
-        -> max_of_prefs__M (max_prefs__M Ms code rules) = (Ms', label, o)
-        -> max_of_prefs (max_prefs code rules) = (label, o).
+        -> max_of_prefs__M (max_prefs__M Ms code i rules) = (Ms', label, o)
+        -> ith_suffix orig code i
+        -> max_of_prefs (max_prefs code i rules) = (label, o).
       Proof.
-        intros. destruct (max_prefs code rules) eqn:E; destruct (max_prefs__M Ms code rules) eqn:E1.
+        intros. destruct (max_prefs code i rules) eqn:E;
+                  destruct (max_prefs__M Ms code i rules) eqn:E1.
         - simpl in *. repeat dm; repeat inj_all; subst. eapply mprefs_memo_F in H; eauto.
           + rewrite E in H. subst. simpl in E0. auto.
         - simpl in *. repeat dm; repeat inj_all; subst. eapply mprefs_memo_F in H; eauto.
@@ -216,11 +233,14 @@ Module ImplFn (Import MEM : memo.T).
       Qed.
 
       Lemma acc_recursive_call__M :
-        forall code rules label s l suffix Ms Ms',
+        forall code rules label s l suffix Ms Ms' i i' orig,
           Acc lt (length code)
-          -> lexy_list (zip Ms (map ssnd rules))
+          -> lexy_list orig (zip Ms (map ssnd rules))
           -> length Ms = length rules
-          -> max_of_prefs__M (max_prefs__M Ms code rules) = (Ms', label, Some (s :: l, suffix))
+          -> max_of_prefs__M (max_prefs__M Ms code i rules)
+            = (Ms', label, Some (s :: l, suffix, i'))
+          -> ith_suffix orig code i
+          -> ith_suffix orig suffix i'
           -> Acc lt (length suffix).
       Proof.
         intros. eapply acc_helper__M in H0; eauto; eapply acc_recursive_call; eauto.
@@ -231,10 +251,10 @@ Module ImplFn (Import MEM : memo.T).
 
     Module Export Lengths.
 
-      Lemma memo_len_const : forall n Ms rules code Ms' l0,
+      Lemma memo_len_const : forall n Ms rules code Ms' l0 i,
         n = length Ms'
         -> length Ms = length rules
-        -> max_prefs__M Ms code rules = (Ms', l0)
+        -> max_prefs__M Ms code i rules = (Ms', l0)
         -> length Ms' = length Ms.
       Proof.
         induction n; intros; destruct rules; destruct Ms; destruct Ms'; destruct l0;
@@ -244,10 +264,10 @@ Module ImplFn (Import MEM : memo.T).
           apply cons_mprefs__M in H1. destruct H1. eapply IHn in H2; eauto.
       Qed.
 
-      Lemma labeled_len_const : forall n Ms rules code Ms' l0,
+      Lemma labeled_len_const : forall n Ms rules code Ms' l0 i,
           n = length Ms'
           -> length Ms = length rules
-          -> max_prefs__M Ms code rules = (Ms', l0)
+          -> max_prefs__M Ms code i rules = (Ms', l0)
           -> length Ms' = length l0.
       Proof.
         induction n; intros; destruct rules; destruct Ms; destruct Ms'; destruct l0;
@@ -257,10 +277,10 @@ Module ImplFn (Import MEM : memo.T).
           apply cons_mprefs__M in H1. destruct H1. eapply IHn in H2; eauto.
       Qed.
 
-      Lemma all_lens_const' : forall n Ms rules code Ms' l0,
+      Lemma all_lens_const' : forall n Ms rules code Ms' l0 i,
           n = length Ms'
           -> length Ms = length rules
-          -> max_prefs__M Ms code rules = (Ms', l0)
+          -> max_prefs__M Ms code i rules = (Ms', l0)
           -> length Ms' = length Ms /\ length Ms' = length l0.
       Proof.
         intros. split.
@@ -268,40 +288,41 @@ Module ImplFn (Import MEM : memo.T).
         - eapply labeled_len_const; eauto.
       Qed.
 
-      Lemma all_lens_const : forall Ms rules code Ms' l0,
+      Lemma all_lens_const : forall Ms rules code Ms' l0 i,
           length Ms = length rules
-          -> max_prefs__M Ms code rules = (Ms', l0)
+          -> max_prefs__M Ms code i rules = (Ms', l0)
           -> length Ms' = length Ms /\ length Ms' = length l0.
       Proof.
         intros. eapply all_lens_const'; eauto.
       Qed.
 
       Lemma len_recursive_call :
-        forall code rules label s l suffix Ms Ms',
+        forall code rules label s l suffix Ms Ms' i i',
           length Ms = length rules
-          -> max_of_prefs__M (max_prefs__M Ms code rules) = (Ms', label, Some (s :: l, suffix))
+          -> max_of_prefs__M (max_prefs__M Ms code i rules)
+            = (Ms', label, Some (s :: l, suffix, i'))
           -> length Ms' = length rules.
       Proof.
-        intros. destruct (max_prefs__M Ms code rules) eqn:E.
+        intros. destruct (max_prefs__M Ms code i rules) eqn:E.
         assert(l0 = Ms').
         {
           simpl in H0. repeat dm. injection H0; auto.
         }
         subst. clear H0.
-        assert(L := all_lens_const Ms rules code Ms' l1 H E). destruct L. omega.
+        assert(L := all_lens_const Ms rules code Ms' l1 i H E). destruct L. omega.
       Qed.
       
     End Lengths.
 
     Module Export LexyClosure.
 
-      Lemma nth_labels_match'' : forall m n rules Ms code Ms' l0 o ru label label',
+      Lemma nth_labels_match'' : forall m n rules Ms code Ms' l0 o ru label label' i,
         m = length rules
         -> length Ms = length rules
         -> length rules = length l0
         -> length Ms' = length Ms
         -> n < length Ms'
-        -> max_prefs__M Ms code rules = (Ms', l0)
+        -> max_prefs__M Ms code i rules = (Ms', l0)
         -> nth n l0 ([], None) = (label, o)
         -> nth n rules ([], defState) = (label', ru)
         -> label = label'.
@@ -318,22 +339,22 @@ Module ImplFn (Import MEM : memo.T).
           eapply IHm; eauto.
       Qed.
 
-      Lemma nth_labels_match' : forall m n rules Ms code Ms' l0 o ru label label',
+      Lemma nth_labels_match' : forall m n rules Ms code Ms' l0 o ru label label' i,
           m = length rules
           -> length Ms = length rules
           -> n < length Ms'
-          -> max_prefs__M Ms code rules = (Ms', l0)
+          -> max_prefs__M Ms code i rules = (Ms', l0)
           -> nth n l0 ([], None) = (label, o)
           -> nth n rules ([], defState) = (label', ru)
           -> label = label'.
       Proof.
         intros.
-        assert(L := all_lens_const Ms rules code Ms' l0 H0 H2). destruct L.
+        assert(L := all_lens_const Ms rules code Ms' l0 i H0 H2). destruct L.
         eapply nth_labels_match''; eauto. omega.
       Qed.
 
-      Lemma nth_labels_match : forall n rules Ms code Ms' l0 o ru label label',
-          max_prefs__M Ms code rules = (Ms', l0)
+      Lemma nth_labels_match : forall n rules Ms code Ms' l0 o ru label label' i,
+          max_prefs__M Ms code i rules = (Ms', l0)
           -> length Ms = length rules
           -> n < length Ms'
           -> nth n l0 ([], None) = (label, o)
@@ -344,15 +365,17 @@ Module ImplFn (Import MEM : memo.T).
       Qed.
 
       Lemma mprefs__M_associates :
-        forall n rules Ms Ms' code (l0 : list (Label * option (Prefix * Suffix))) M M' o label ru,
+        forall n rules Ms Ms' code (l0 : list (Label * option (Prefix * Suffix * index)))
+          M M' o label ru i,
           length Ms = length rules
-          -> max_prefs__M Ms code rules = (Ms', l0)
+          -> max_prefs__M Ms code i rules =
+            (Ms', l0)
           -> n < length Ms'
           -> nth n Ms emptyMemo = M
           -> nth n Ms' emptyMemo = M'
           -> nth n l0 ([], None) = (label, o)
           -> nth n rules ([], defState) = (label, ru)
-          -> max_pref_fn__M M code ru = (M', o).
+          -> max_pref_fn__M M code i ru = (M', o).
       Proof.
         induction n; intros; destruct Ms; destruct Ms'; destruct l0; destruct rules;
           try(simpl in *; omega);
@@ -365,42 +388,77 @@ Module ImplFn (Import MEM : memo.T).
           apply lt_S_n in H1. eapply IHn; eauto. eapply cons_mprefs__M; eauto.
       Qed.
 
-      Lemma set_Memo_lexy : forall z z0 o o' p p0 d m,
-          max_pref_fn z (p, d) = o'
-          -> lexy m d
-          -> get_Memo (set_Memo m p z o') p0 z0 = Some o
-          -> max_pref_fn z0 (p0, d) = o.
+      Lemma app_cons_comm2 : forall {A : Type} xs ys (y : A),
+          xs ++ y :: ys = (xs ++ [y]) ++ ys.
+      Admitted.
+
+      Lemma eq_len_suffix : forall {A : Type} (z0 z x0 x : list A),
+          x0 ++ z0 = x ++ z
+          -> length z = length z0
+          -> x0 = x /\  z0 = z.
+      Proof.
+        induction z0; destruct z; intros; sis; auto; try(discriminate).
+        - split; auto. do 2 rewrite <- app_nil_end in *. auto.
+        - do 2 (rewrite app_cons_comm2 in H; symmetry in H).
+          apply IHz0 in H; auto. destruct H. subst.
+          assert(rev (x0 ++ [a]) = rev (x ++ [a0])).
+          { apply f_equal. auto. }
+          do 2 rewrite rev_unit in *. inv H1.
+          assert(rev (rev x0) = rev (rev x)).
+          { apply f_equal. auto. }
+          do 2 rewrite rev_involutive in *. subst. auto.
+      Qed.
+
+      Lemma set_Memo_lexy : forall z z0 o o' p p0 d m code i i0,
+          max_pref_fn z i (p, d) = o'
+          -> lexy code m d
+          -> get_Memo (set_Memo m p i o') p0 i0 = Some o
+          -> ith_suffix code z i
+          -> ith_suffix code z0 i0
+          -> max_pref_fn z0 i0 (p0, d) = o.
       Proof.
         intros. destruct (String_dec z z0).
         (* originally tried to find an ordering on State *)
         (* realized that was too much, tried to find decidable equality *)
         (* seems like even that is too much, considering that 
            the Table and final states doesn't change, only the state-pointer *)
-        - subst. destruct (pointer_compare p p0) eqn:E.
+        - rewrite e in *. clear e.
+          assert(i = i0).
+          { unfold ith_suffix in *. destruct H2. destruct H3. destruct H4. destruct H5.
+            subst. auto. }
+          rewrite H4 in *. clear H4. clear i.
+          subst. destruct (pointer_compare p p0) eqn:E.
           + apply pointer_compare_eq in E. subst. rewrite correct_Memo in H1. inv H1. auto.
           + assert(p <> p0).
             { intros C. apply pointer_compare_eq in C. rewrite C in *. discriminate. }
             clear E.
-            assert(p0 <> p \/ z0 <> z0); auto.
-            eapply correct_Memo_moot in H2; eauto. rewrite H2 in H1.
+            assert(p0 <> p \/ i0 <> i0); auto.
+            eapply correct_Memo_moot in H4; eauto. rewrite H4 in H1.
             eapply lexy_correct; eauto.
           + assert(p <> p0).
             { intros C. apply pointer_compare_eq in C. rewrite C in *. discriminate. }
             clear E.
-            assert(p0 <> p \/ z0 <> z0); auto.
-            eapply correct_Memo_moot in H2; eauto. rewrite H2 in H1.
+            assert(p0 <> p \/ i0 <> i0); auto.
+            eapply correct_Memo_moot in H4; eauto. rewrite H4 in H1.
             eapply lexy_correct; eauto.
-        - assert(p0 <> p \/ z0 <> z); auto.
-          clear n. eapply correct_Memo_moot in H2; eauto. rewrite H2 in H1.
+        - assert(i <> i0).
+          { intros C. destruct n. unfold ith_suffix in *.
+            destruct H2. destruct H3. destruct H4. destruct H5.
+            subst. apply n_det_index in C. apply eq_len_suffix in H5; auto. destruct H5. auto. }
+           assert(p0 <> p \/ i0 <> i); auto.
+          clear n. eapply correct_Memo_moot in H5; eauto. rewrite H5 in H1.
           eapply lexy_correct; eauto.
       Qed.
 
       Lemma lexy_closure : 
-        forall code p d M o M',
-          lexy M d
-          -> max_pref_fn__M M code (p,d) = (M', o)
-          -> lexy M' d.
+        forall code p d M o M' i orig,
+          lexy orig M d
+          -> max_pref_fn__M M code i (p,d) = (M', o)
+          -> ith_suffix orig code i
+          -> lexy orig M' d.
       Proof.
+      Admitted.
+        (*
         induction code; intros.
         {
           simpl in H0. dm; inv H0; auto.
@@ -439,82 +497,85 @@ Module ImplFn (Import MEM : memo.T).
             eapply set_Memo_lexy; eauto.
         }
       Qed.
+         *)
 
       
 
       Lemma lexy_list_closure : 
-        forall code rules Ms l0 Ms',
-          lexy_list (zip Ms (map ssnd rules))
+        forall code rules Ms l0 Ms' i orig,
+          lexy_list orig (zip Ms (map ssnd rules))
           -> length Ms = length rules
-          -> max_prefs__M Ms code rules = (Ms', l0)
-          -> lexy_list (zip Ms' (map ssnd rules)).
+          -> max_prefs__M Ms code i rules = (Ms', l0)
+          -> ith_suffix orig code i
+          -> lexy_list orig (zip Ms' (map ssnd rules)).
       Proof.
-        intros. unfold lexy_list in *. intros M' d H2.
-        apply In_nth with (d := (emptyMemo, defDelta)) in H2. destruct H2 as [n]. destruct H2.
-        assert(L := all_lens_const Ms rules code Ms' l0 H0 H1). destruct L.
+        intros. unfold lexy_list in *. intros M' d H3.
+        apply In_nth with (d := (emptyMemo, defDelta)) in H3. destruct H3 as [n]. destruct H3.
+        assert(L := all_lens_const Ms rules code Ms' l0 i H0 H1). destruct L.
         assert(exists M, nth n Ms emptyMemo = M).
         { eexists; eauto. }
-        destruct H6 as [M].
+        destruct H7 as [M].
         assert(exists label o, nth n l0 ([], None) = (label, o)).
         { destruct (nth n l0 ([], None)). eexists; eauto. }
-        destruct H7 as [label]. destruct H7 as [o].
+        destruct H8 as [label]. destruct H8 as [o].
         assert(exists label' ru, nth n rules ([], defState) = (label', ru)).
         { destruct (nth n rules ([], defState)). eexists; eauto. }
-        destruct H8 as [label']. destruct H8 as [ru].
+        destruct H9 as [label']. destruct H9 as [ru].
         assert(label = label').
         {
-          eapply nth_labels_match; eauto. rewrite len_zip_L in H2; auto.
+          eapply nth_labels_match; eauto. rewrite len_zip_L in H3; auto.
           rewrite map_length. omega.
         }
-        rewrite H9 in *. clear H9.
+        rewrite H10 in *. clear H10.
         rewrite nth_zip in *.
         assert(nth n (zip Ms (map (fun x : Label * (Pointer * Delta) => snd (snd x)) rules))
                    (emptyMemo, defDelta) = (M, d)).
         {
           rewrite nth_zip.
-          - inv H3. auto.
+          - inv H4. auto.
           - rewrite map_length. omega.
-          - rewrite len_zip_L in H2; try omega. rewrite map_length. omega.
+          - rewrite len_zip_L in H3; try omega. rewrite map_length. omega.
         }
         assert(n < length (zip Ms (map (fun x : Label * (Pointer * Delta) => snd (snd x)) rules))).
         {
-          rewrite len_zip_L; [ rewrite len_zip_L in H2 | ]; try rewrite map_length; omega.
+          rewrite len_zip_L; [ rewrite len_zip_L in H3 | ]; try rewrite map_length; omega.
         }
         eapply mprefs__M_associates in H0; eauto.
         - destruct ru.
           assert(d = d0).
           {
-            injection H3; intros.
-            clear H H1 H2 H3 H4 H5 H6 H7 H9 H10 H12 H0 code Ms l0.
+            injection H4; intros.
+            clear H H1 H2 H3 H4 H5 H6 H7 H8 H10 H11 H13 H0 code Ms l0.
             unfold defState.
             assert(exists x, nth n rules (x, (defPointer, defDelta)) = (label', (p, d0))).
             { eexists; eauto. }
-            clear H8. destruct H as (x & H).
+            clear H9. destruct H as (x & H).
             assert(defDelta = ssnd (x, (defPointer, defDelta))).
             { auto. }
-            rewrite H0 in H11. rewrite map_nth in H11. rewrite H in H11.
+            rewrite H0 in H12. rewrite map_nth in H12. rewrite H in H12.
             unfold ssnd in *. sis. auto.
           }
           subst.
           assert(In (nth n Ms emptyMemo, d0)
                     (zip Ms (map (fun x : Label * (Pointer * Delta) => snd (snd x)) rules))).
           {
-            eapply nth_In in H10. rewrite H9 in H10. auto.
+            eapply nth_In in H11. rewrite H10 in H11. auto.
           }
-          inv H3. apply H in H6. eapply lexy_closure; eauto.
-        - rewrite len_zip_L in H2; auto. rewrite map_length. omega.
+          inv H4. eapply lexy_closure; eauto.
+        - rewrite len_zip_L in H3; auto. rewrite map_length. omega.
         - rewrite map_length. omega.
-        - rewrite len_zip_L in H2; try omega. rewrite map_length. omega.
+        - rewrite len_zip_L in H3; try omega. rewrite map_length. omega.
       Qed.
 
       Lemma lexy_recursive_call_gen :
-        forall code rules Ms label o Ms',
-          lexy_list (zip Ms (map (fun x => snd (snd x)) rules))
+        forall code rules Ms label o Ms' i orig,
+          lexy_list orig (zip Ms (map (fun x => snd (snd x)) rules))
           -> length Ms = length rules
-          -> max_of_prefs__M (max_prefs__M Ms code rules) = (Ms', label, o)
-          -> lexy_list (zip Ms' (map (fun x => snd (snd x)) rules)).
+          -> max_of_prefs__M (max_prefs__M Ms code i rules) = (Ms', label, o)
+          -> ith_suffix orig code i
+          -> lexy_list orig (zip Ms' (map (fun x => snd (snd x)) rules)).
       Proof.
-        intros. destruct (max_prefs__M Ms code rules) eqn:E.
+        intros. destruct (max_prefs__M Ms code i rules) eqn:E.
         assert(l = Ms').
         {
           simpl in H1. repeat dm. injection H1; auto.
@@ -524,39 +585,72 @@ Module ImplFn (Import MEM : memo.T).
       Qed.
 
       Lemma lexy_recursive_call :
-        forall code rules Ms label s l suffix Ms',
-          lexy_list (zip Ms (map (fun x => snd (snd x)) rules))
+        forall code rules Ms label s l suffix Ms' i i' orig,
+          lexy_list orig (zip Ms (map (fun x => snd (snd x)) rules))
           -> length Ms = length rules
-          -> max_of_prefs__M (max_prefs__M Ms code rules) = (Ms', label, Some (s :: l, suffix))
-          -> lexy_list (zip Ms' (map (fun x => snd (snd x)) rules)).
+          -> max_of_prefs__M (max_prefs__M Ms code i rules)
+            = (Ms', label, Some (s :: l, suffix, i'))
+          -> ith_suffix orig code i
+          -> ith_suffix orig suffix i'
+          -> lexy_list orig (zip Ms' (map (fun x => snd (snd x)) rules)).
+      Proof.
         intros. eapply lexy_recursive_call_gen in H; eauto.
       Qed.
 
     End LexyClosure.
+
+    Module Export IndexClosure.
+
+      Lemma index_rec_call__M : forall code rules Ms label s l suffix Ms' i i' orig,
+           lexy_list orig (zip Ms (map ssnd rules))
+           -> length Ms = length rules
+           -> max_of_prefs__M (max_prefs__M Ms code i rules) = (Ms', label, Some (s :: l, suffix, i'))
+           -> ith_suffix orig code i
+           -> ith_suffix orig suffix i'.
+      Proof.
+        
+        intros.
+        destruct (max_prefs__M Ms code i rules) eqn:E. eapply mprefs_memo_F in E; eauto.
+        rewrite <- E in H1. unfold max_of_prefs__M in *. dm. inv H1.
+        unfold ith_suffix in *. destruct H2. destruct H2.
+        split.
+        - apply index_rec_call in E0; auto.
+        - exists (x ++ (s :: l)). rewrite <- app_assoc. rewrite <- H1 in *.
+          apply exists_rus_of_mpref_gen in E0. destruct E0 as (r & HIn & E0).
+          symmetry in E0. apply max_pref_fn_splits in E0. rewrite <- E0. auto.
+      Defined.
+          
+
+    End IndexClosure.
     
   End TypeCheckLemmas.
 
   Module Export Lex.
 
     Fixpoint lex'__M
+             (orig : String)
              (Ms : list Memo)
              (rules : list (sRule))
              (code : String)
+             (i : index)
+             (Hindex : ith_suffix orig code i)
              (Ha : Acc lt (length code))
-             (Hlexy : lexy_list (zip Ms (map ssnd rules)))
+             (Hlexy : lexy_list orig (zip Ms (map ssnd rules)))
              (Hlen : length Ms = length rules)
              {struct Ha} : (list Memo) * (list Token) * String :=
-      match max_of_prefs__M (max_prefs__M Ms code rules) as mpref'
-            return max_of_prefs__M (max_prefs__M Ms code rules) = mpref' -> _
+      match max_of_prefs__M (max_prefs__M Ms code i rules) as mpref'
+            return max_of_prefs__M (max_prefs__M Ms code i rules) = mpref' -> _
       with
       | (Ms', _, None) => fun _ => (Ms', [], code) (* Code cannot be processed further *)
-      | (Ms', _, Some ([], _)) => fun _ => (Ms', [], code) (* Code cannot be processed further *)
-      | (Ms', label, Some (ph :: pt, suffix)) =>
+      | (Ms', _, Some ([], _, _)) => fun _ => (Ms', [], code) (* Code cannot be processed further *)
+      | (Ms', label, Some (ph :: pt, suffix, i')) =>
         fun Heq =>
-          match (lex'__M Ms' rules suffix
-                       (acc_recursive_call__M _ _ _ _ _ _ _ _ Ha Hlexy Hlen Heq)
-                       (lexy_recursive_call _ _ _ _ _ _ _ _ Hlexy Hlen Heq)
-                       (len_recursive_call _ _ _ _ _ _ _ _ Hlen Heq)
+          let Hindex' := (index_rec_call__M _ _ _ _ _ _ _ _ _ _ _ Hlexy Hlen Heq Hindex) in
+          match (lex'__M orig Ms' rules suffix i'
+                       Hindex'
+                       (acc_recursive_call__M _ _ _ _ _ _ _ _ _ _ _ Ha Hlexy Hlen Heq Hindex Hindex')
+                       (lexy_recursive_call _ _ _ _ _ _ _ _ _ _ _ Hlexy Hlen Heq Hindex Hindex')
+                       (len_recursive_call _ _ _ _ _ _ _ _ _ _ Hlen Heq)
                 )
           with
           | (Ms'', lexemes, rest) => (Ms'', ((label, ph :: pt) :: lexemes), rest)
@@ -571,16 +665,16 @@ Module ImplFn (Import MEM : memo.T).
     Definition init_Memos (srules : list sRule) : list Memo :=
       (map (fun x => emptyMemo) srules).
 
-    Lemma lexy_list_cons : forall M Ms d,
-        lexy M d -> lexy_list Ms -> lexy_list ((M, d) :: Ms).
+    Lemma lexy_list_cons : forall M Ms d code,
+        lexy code M d -> lexy_list code Ms -> lexy_list code ((M, d) :: Ms).
     Proof.
       intros. unfold lexy_list in *. intros. sis. destruct H1.
       - inv H1. auto.
       - apply H0; auto.
     Qed.
 
-    Lemma init_Memos_lexy : forall srules,
-        lexy_list (zip (init_Memos srules) (map ssnd srules)).
+    Lemma init_Memos_lexy : forall srules code,
+        lexy_list code (zip (init_Memos srules) (map ssnd srules)).
     Proof.
       intros. induction srules.
       - simpl. unfold lexy_list. intros. contradiction.
@@ -594,13 +688,19 @@ Module ImplFn (Import MEM : memo.T).
       intros. induction srules; auto. sis. omega.
     Qed.
 
+    Lemma init_index_self : forall code,
+        ith_suffix code code (init_index (length code)).
+    Proof.
+      intros. split; auto. exists []. auto.
+    Qed.
+
     Definition lex__M (rules : list Rule) (code : String) : list Token * String :=
       let
         srules := map init_srule rules
       in
       match
-        lex'__M (init_Memos srules) srules code
-              (lt_wf _) (init_Memos_lexy _) (init_Memos_parallel _)
+        lex'__M code (init_Memos srules) srules code (init_index (length code))
+              (init_index_self _) (lt_wf _) (init_Memos_lexy _ _) (init_Memos_parallel _)
        with
        | (_, ts, rest) => (ts, rest)
        end.
