Verbatim/lexer/lemmas.v
@@ -18,39 +18,43 @@ Module LemmasFn (Import ST : state.T).
   Import MatchSpec.
 
   Lemma lex'_eq_body :
-    forall rules code (Ha : Acc lt (length code)),
-      (lex' rules code Ha =
-       (match max_of_prefs (max_prefs code rules) as mpref'
-              return max_of_prefs (max_prefs code rules) = mpref' -> _
+    forall rules code i (Hindex : i = init_index (length code)) (Ha : Acc lt (length code)),
+      (lex' rules code i Hindex Ha =
+       (match max_of_prefs (max_prefs code i rules) as mpref'
+              return max_of_prefs (max_prefs code i rules) = mpref' -> _
         with
         | (_, None) => fun _ => ([], code) (* Code cannot be processed further *)
-        | (_, Some ([], _)) => fun _ => ([], code) (* Code cannot be processed further *)
-        | (label, Some (ph :: pt, suffix)) =>
+        | (_, Some ([], _, _)) => fun _ => ([], code) (* Code cannot be processed further *)
+        | (label, Some (ph :: pt, suffix, i')) =>
           fun Heq =>
-            match (lex' rules suffix
-                        (acc_recursive_call _ _ _ _ _ _ Ha Heq))
+            match (lex' rules suffix i'
+                        (index_rec_call _ _ _ _ _ _ _ _ Hindex Heq)
+                        (acc_recursive_call _ _ _ _ _ _ _ _ Ha Heq))
             with
             | (lexemes, rest) => (((label, ph :: pt) :: lexemes), rest)
             end
         end eq_refl)).
   Proof.
-    intros rules code Ha. unfold lex'. destruct Ha. auto.
+    intros rules code i Hindex Ha. unfold lex'. destruct Ha. auto.
   Qed.
 
   Lemma lex'_cases_backward :
     forall (rules : list sRule)
       (code : String)
+      (i : index)
+      (Hindex : i = init_index (length code))
       (Ha : Acc lt (length code))
-      (pr : Label * option (Prefix * Suffix))
+      (pr : Label * option (Prefix * Suffix * index))
       (res : list Token * String)
-      (Heq : max_of_prefs (max_prefs code rules) = pr),
-      match pr as mpref' return max_of_prefs (max_prefs code rules) = mpref' -> _ with
+      (Heq : max_of_prefs (max_prefs code i rules) = pr),
+      match pr as mpref' return max_of_prefs (max_prefs code i rules) = mpref' -> _ with
       | (_, None) => fun _ => ([], code) (* Code cannot be processed further *)
-      | (_, Some ([], _)) => fun _ => ([], code) (* Code cannot be processed further *)
-      | (label, Some (h :: t, suffix)) =>
+      | (_, Some ([], _, _)) => fun _ => ([], code) (* Code cannot be processed further *)
+      | (label, Some (h :: t, suffix, i')) =>
         fun Heq =>
-          match (lex' rules suffix
-                      (acc_recursive_call _ _ _ _ _ _ Ha Heq))
+          match (lex' rules suffix i'
+                      (index_rec_call _ _ _ _ _ _ _ _ Hindex Heq)
+                      (acc_recursive_call _ _ _ _ _ _ _ _ Ha Heq))
           with
           | (lexemes, rest) => (((label, h :: t) :: lexemes), rest)
           end
@@ -59,35 +63,41 @@ Module LemmasFn (Import ST : state.T).
         | ([], code') =>
           code' = code
           /\ (snd pr = None
-             \/ exists suf, snd pr = Some ([], suf))
+             \/ exists suf i', snd pr = Some ([], suf, i'))
         | ((label, prefix) :: lexemes, rest) =>
-          exists h t suffix (Heq' : max_of_prefs (max_prefs code rules) = (label, Some (h :: t, suffix))),
-          lex' rules suffix (acc_recursive_call _ _ _ _ _ _ Ha Heq') = (lexemes, rest)
+          exists h t suffix i' (Heq' : max_of_prefs (max_prefs code i rules)
+                               = (label, Some (h :: t, suffix, i'))),
+          lex' rules suffix i'
+               (index_rec_call _ _ _ _ _ _ _ _ Hindex Heq')
+               (acc_recursive_call _ _ _ _ _ _ _ _ Ha Heq') = (lexemes, rest)
           /\ h :: t = prefix
         end.
   Proof.
-    intros rules code Ha pr res Heq.
+    intros.
     repeat dm; intros; subst; simpl in *; try congruence.
     - split; inv H; eauto.
-    - inv H. exists s0. exists p1. exists s. exists Heq. split. apply E3. reflexivity.
+    - inv H. exists s0. exists p2. exists s. exists i0. exists Heq. split; auto.
     - split; inv H; eauto.
   Qed.
 
   Lemma lex'_cases :
-    forall rules code Ha res,
-      lex' rules code Ha = res
+    forall rules code i Hindex Ha res,
+      lex' rules code i Hindex Ha = res
       -> match res with
         | ([], code') =>
           code' = code
-          /\ (snd (max_of_prefs (max_prefs code rules)) = None
-             \/ exists suf, snd (max_of_prefs (max_prefs code rules)) = Some ([], suf))
+          /\ (snd (max_of_prefs (max_prefs code i rules)) = None
+             \/ exists suf i', snd (max_of_prefs (max_prefs code i rules)) = Some ([], suf, i'))
         | ((label, prefix) :: lexemes, rest) =>
-          exists h t suffix (Heq' : max_of_prefs (max_prefs code rules) = (label, Some (h :: t, suffix))),
-          lex' rules suffix (acc_recursive_call _ _ _ _ _ _ Ha Heq') = (lexemes, rest)
+          exists h t suffix i' (Heq' : max_of_prefs (max_prefs code i rules)
+                               = (label, Some (h :: t, suffix, i'))),
+          lex' rules suffix i'
+               (index_rec_call _ _ _ _ _ _ _ _ Hindex Heq')               
+               (acc_recursive_call _ _ _ _ _ _ _ _ Ha Heq') = (lexemes, rest)
           /\ h :: t = prefix
         end.
   Proof.
-    intros rules code Ha res Heq; subst.
+    intros; subst.
     rewrite lex'_eq_body.
     eapply lex'_cases_backward; eauto.
   Qed.
@@ -169,18 +179,16 @@ Module LemmasFn (Import ST : state.T).
   Qed.
 
   
-  Lemma mpref_cons : forall code px sx fsm a,
-      max_pref_fn code (transition a fsm) = Some (px, sx)
-      <-> max_pref_fn (a :: code) fsm = Some (a :: px, sx).
+  Lemma mpref_cons : forall code px sx fsm a i i',
+      max_pref_fn code i (transition a fsm) = Some (px, sx, i')
+      <-> max_pref_fn (a :: code) (incr i) fsm = Some (a :: px, sx, i').
   Proof.
-    intros. simpl. repeat dm; split; intros; try(discriminate).
-    - injection H; intros; subst; reflexivity.
-    - injection H; intros; subst; reflexivity.
-    - clear H. exfalso.
-      destruct code.
-      + simpl in E. dm; try(discriminate).
-      + simpl in E. repeat dm; try(discriminate).
+    intros. simpl.
+    repeat dm; split; intros;
+      try( rewrite decr_inv_incr in *; rewrite E in *; repeat inj_all; auto; discriminate ).
+    destruct code; sis; repeat dm; discriminate.
   Qed.
+        
 
   Lemma accepting_dt : forall b e,
       accepting (transition b (init_state e)) =
@@ -209,12 +217,12 @@ Module LemmasFn (Import ST : state.T).
   Proof. auto. Qed.
 
   (* ow *)
-  Lemma mpref_dt_list : forall code bs e a,
-      max_pref_fn code (transition a (init_state e))
-      = max_pref_fn code (init_state (derivative a e))
+  Lemma mpref_dt_list : forall code bs e a i,
+      max_pref_fn code i (transition a (init_state e))
+      = max_pref_fn code i (init_state (derivative a e))
       /\
-      max_pref_fn code (transition_list bs (init_state e)) =
-      max_pref_fn code (init_state (derivative_list bs e)).
+      max_pref_fn code i (transition_list bs (init_state e)) =
+      max_pref_fn code i (init_state (derivative_list bs e)).
   Proof.
     induction code; induction bs; intros.
     - split; auto; simpl; repeat dm.
@@ -235,48 +243,30 @@ Module LemmasFn (Import ST : state.T).
           rewrite <- derivative_list_cons in *.
           rewrite <- accepting_dt_list in *. rewrite transition_list_cons in *.
           rewrite E in *. discriminate.
-    - assert(IHcode0 : forall (e : regex) (a : Sigma),
-           max_pref_fn code (transition a (init_state e)) =
-           max_pref_fn code (init_state (derivative a e))).
+    - assert(IHcode0 : forall (e : regex) (a : Sigma) i,
+           max_pref_fn code i (transition a (init_state e)) =
+           max_pref_fn code i (init_state (derivative a e))).
       { intros. specialize (IHcode []). apply IHcode. }
-      assert(IHcode1 : forall (bs : list Sigma) (e : regex),
-           max_pref_fn code (transition_list bs (init_state e)) =
-           max_pref_fn code (init_state (derivative_list bs e))).
+      assert(IHcode1 : forall (bs : list Sigma) (e : regex) i,
+           max_pref_fn code i (transition_list bs (init_state e)) =
+           max_pref_fn code i (init_state (derivative_list bs e))).
       { intros. specialize (IHcode bs e0 a). apply IHcode. }
       clear IHcode.
       split.
-      + destruct (max_pref_fn (a :: code) (transition a0 (init_state e))) eqn:E.
+      + destruct (max_pref_fn (a :: code) i (transition a0 (init_state e))) eqn:E.
         * destruct p. symmetry.
           destruct p.
-          -- simpl in *. repeat dm; try(discriminate).
-             ++ rewrite IHcode0 in E3.
-                rewrite dbl_trans_lst in E0.
-                rewrite dbl_deriv_lst in E3.
-                rewrite IHcode1 in *. rewrite E3 in *. discriminate.
-             ++ exfalso.
-                clear IHcode0 IHcode1 E0 E2 E E3.
-                rewrite dbl_trans_lst in *.
-                assert(
-                    accepting (transition a (init_state (derivative a0 e)))
-                    = accepting (transition_list [a] (init_state (derivative a0 e)))
-                  ).
-                { rewrite transition_list_cons. rewrite transition_list_nil. auto. }
-                rewrite H in *. clear H.
-                rewrite accepting_dt_list in *.
-                simpl in *. rewrite E1 in *. discriminate.
-             ++ rewrite accepting_dt in *. rewrite E5 in *. discriminate.
-          -- assert(a = s0).
-             {
-               simpl in E.
-               repeat dm; try(discriminate);
-                 injection E; intros; subst; auto.
-             }
-             subst.
-             rewrite <- mpref_cons. rewrite <- mpref_cons in E.
-             rewrite IHcode0.
-             rewrite dbl_trans_lst in *.
-             rewrite dbl_deriv_lst in *.
-             rewrite <- IHcode1. auto.
+          simpl in *.
+          repeat dm; try(discriminate); repeat inj_all;
+            try( rewrite IHcode0 in *;
+                 rewrite dbl_trans_lst in *;
+                 rewrite dbl_deriv_lst in *;
+                 rewrite IHcode1 in *);
+                 try(rewrite E3 in *; repeat inj_all; auto; discriminate);
+                 try(rewrite E0 in *; repeat inj_all; auto; discriminate);
+                 try(rewrite accepting_dt in *; rewrite accepting_dt_list in *; sis; auto);
+                 try(rewrite E1 in *; discriminate).
+                 rewrite E2 in *. discriminate.
         * simpl in *. repeat dm; try(discriminate).
           -- clear E. rewrite IHcode0 in E3. 
              rewrite dbl_trans_lst in E0.
@@ -289,85 +279,43 @@ Module LemmasFn (Import ST : state.T).
              rewrite E4 in *. discriminate.
           -- rewrite accepting_dt in *. rewrite E5 in *. discriminate.       
       + rewrite transition_list_nil. unfold derivative_list. auto.
-    - assert(IHcode0 : forall (e : regex) (a : Sigma),
-           max_pref_fn code (transition a (init_state e)) =
-           max_pref_fn code (init_state (derivative a e))).
+    - assert(IHcode0 : forall (e : regex) (a : Sigma) i,
+           max_pref_fn code i (transition a (init_state e)) =
+           max_pref_fn code i (init_state (derivative a e))).
       { intros. specialize (IHcode []). apply IHcode. }
-      assert(IHcode1 : forall (bs : list Sigma) (e : regex),
-           max_pref_fn code (transition_list bs (init_state e)) =
-           max_pref_fn code (init_state (derivative_list bs e))).
+      assert(IHcode1 : forall (bs : list Sigma) (e : regex) i,
+           max_pref_fn code i (transition_list bs (init_state e)) =
+           max_pref_fn code i (init_state (derivative_list bs e))).
       { intros. specialize (IHcode bs0 e0 a). apply IHcode. }
       clear IHcode.
-      assert(IHbs0 : forall (e : regex) (a0 : Sigma),
-         max_pref_fn (a :: code) (transition a0 (init_state e)) =
-         max_pref_fn (a :: code) (init_state (derivative a0 e))).
+      assert(IHbs0 : forall (e : regex) (a0 : Sigma) i,
+         max_pref_fn (a :: code) i (transition a0 (init_state e)) =
+         max_pref_fn (a :: code) i (init_state (derivative a0 e))).
       { intros. apply IHbs. }
-      assert(IHbs1 : forall (e : regex) (a0 : Sigma),
-         max_pref_fn (a :: code) (transition_list bs (init_state e)) =
-         max_pref_fn (a :: code) (init_state (derivative_list bs e))).
+      assert(IHbs1 : forall (e : regex) (a0 : Sigma) i,
+         max_pref_fn (a :: code) i (transition_list bs (init_state e)) =
+         max_pref_fn (a :: code) i (init_state (derivative_list bs e))).
       { intros. apply IHbs. apply a. }
       clear IHbs.
       split.
       + auto.
-      + destruct (max_pref_fn (a :: code) (transition_list (a0 :: bs) (init_state e))) eqn:E.
+      + destruct (max_pref_fn (a :: code) i (transition_list (a0 :: bs) (init_state e))) eqn:E.
         * destruct p. destruct p.
-          -- simpl in E. simpl. repeat dm; try(discriminate).
-             ++ rewrite IHcode0 in *.
-                rewrite transition_list_cons in *.
-                rewrite <- derivative_list_cons in *.
-                rewrite transition_list_hop in *.
-                rewrite deriv_list_hop in *.
-                rewrite <- IHcode1 in *. rewrite <- transition_list_cons in *. sis.
-                rewrite E3 in *. discriminate.
-             ++ rewrite accepting_dt in *.
-                rewrite transition_list_cons in *.
-                rewrite <- derivative_list_cons in *.
-                rewrite transition_list_hop in *.
-                rewrite deriv_list_hop in *.
-                rewrite <- accepting_dt_list in *. sis. rewrite transition_list_cons in *.
-                rewrite E4 in *. discriminate.
-             ++ rewrite transition_list_cons in *.
-                rewrite <- derivative_list_cons in *.
-                rewrite <- accepting_dt_list in *. rewrite transition_list_cons in *.
-                rewrite E5 in *. discriminate.
-          -- simpl in E. simpl.
-             repeat dm; try(discriminate);
-               try(injection E; intros; subst;
-                rewrite IHcode0 in *; rewrite transition_list_hop in E0;
-                rewrite <- transition_cons in E0; rewrite IHcode1 in E0;
-                rewrite derivative_list_cons in E0; rewrite <- deriv_list_hop in E0;
-                rewrite E0 in E2; discriminate);
-               try(injection E; intros; subst;
-                rewrite IHcode0 in *; rewrite transition_list_hop in E0;
-                rewrite <- transition_cons in E0; rewrite IHcode1 in E0;
-                rewrite derivative_list_cons in E0; rewrite <- deriv_list_hop in E0;
-                rewrite E0 in E2; injection E2; intros; subst; reflexivity).
-             ++ rewrite IHcode0 in E2.
-                rewrite transition_list_hop in *.
-                rewrite deriv_list_hop in *.
-                subst. inv E. rewrite IHcode1 in *. sis. rewrite E0 in E2. inv E2. auto.
-             ++ rewrite IHcode0 in E2.
-                rewrite transition_list_hop in *.
-                rewrite deriv_list_hop in *.
-                subst. inv E. rewrite IHcode1 in *. sis. rewrite E0 in E2. inv E2.
-             ++ rewrite IHcode0 in E2.
-                rewrite transition_list_hop in *.
-                rewrite deriv_list_hop in *.
-                subst. inv E. rewrite IHcode1 in *. sis. rewrite E0 in E2. inv E2.
-             ++ rewrite IHcode0 in E2.
-                rewrite transition_list_hop in *.
-                rewrite deriv_list_hop in *.
-                subst. inv E. rewrite IHcode1 in *. sis. rewrite E0 in E2. inv E2.
-             ++ rewrite IHcode0 in E2.
-                rewrite transition_list_hop in *.
-                rewrite deriv_list_hop in *.
-                subst. inv E. rewrite IHcode1 in *. sis. rewrite E0 in E2. inv E2.
-             ++ rewrite accepting_dt in *. rewrite transition_list_hop in *.
-                rewrite accepting_dt_list in *. rewrite <- app_comm_cons in *.
-                rewrite deriv_list_hop in *. sis. rewrite E1 in E3. discriminate.
-             ++ rewrite accepting_dt in *. rewrite transition_list_hop in *.
-                rewrite accepting_dt_list in *. rewrite <- app_comm_cons in *.
-                rewrite deriv_list_hop in *. sis. rewrite E1 in E3. discriminate.
+          simpl in E. simpl. repeat dm; try(discriminate);
+          try(rewrite IHcode0 in *;
+             rewrite transition_list_cons in *;
+             rewrite <- derivative_list_cons in *;
+             rewrite transition_list_hop in *;
+             rewrite deriv_list_hop in *;
+             rewrite <- IHcode1 in *; rewrite <- transition_list_cons in *; sis;
+             rewrite E3 in *; repeat inj_all; auto; discriminate);
+            try(rewrite IHcode0 in *; rewrite <- derivative_list_cons in *;
+             rewrite deriv_list_hop in *; rewrite <- IHcode1 in *;
+             rewrite transition_list_hop in *; rewrite E0 in *; discriminate);
+          try(rewrite accepting_dt in *; rewrite <- derivative_list_cons in *;
+             rewrite deriv_list_hop in *; rewrite <- accepting_dt_list in *;
+             rewrite transition_list_hop in *; rewrite E1 in *; discriminate).
+          rewrite accepting_dt_list in *. sis. rewrite E2 in *. discriminate.
         * simpl in E. simpl. repeat dm; try(discriminate).
           -- rewrite IHcode0 in E3.
              rewrite transition_list_hop in *.
@@ -382,18 +330,22 @@ Module LemmasFn (Import ST : state.T).
   Qed.
         
   
-  Lemma mpref_dt : forall code a e,
-      max_pref_fn code (transition a (init_state e))
-      = max_pref_fn code (init_state (derivative a e)).
+  Lemma mpref_dt : forall code a e i,
+      max_pref_fn code i (transition a (init_state e))
+      = max_pref_fn code i (init_state (derivative a e)).
   Proof.
     assert(L := mpref_dt_list).
-    intros. specialize(L code [] e a). destruct L. auto.
+    intros. specialize(L code [] e a i). destruct L. auto.
   Qed.
 
+  Lemma index_incr_cons : forall (code : String) a,
+      init_index (length (a :: code)) = incr (init_index (length code)).
+  Proof.
+    intros. sis. apply incr_is_S.
+  Qed.
   
-  
-  Lemma max_pref_matches : forall(code p x : String) (e : regex),
-      Some (p, x) = max_pref_fn code (init_state e)
+  Lemma max_pref_matches : forall(code p x : String) (e : regex) i,
+      Some (p, x, i) = max_pref_fn code (init_index (length code)) (init_state e)
       -> exp_match p e.
   Proof.
     induction code; intros.
@@ -407,7 +359,8 @@ Module LemmasFn (Import ST : state.T).
         * rewrite accepts_nil in E1. symmetry in E1. rewrite accepts_matches in E1. auto.
         * discriminate.
       + destruct (Sigma_dec a s).
-        * subst. apply mpref_cons in H. symmetry in H. rewrite mpref_dt in H. apply IHcode in H.
+        * subst. rewrite index_incr_cons in *. apply mpref_cons in H.
+          symmetry in H. rewrite mpref_dt in H. apply IHcode in H.
           apply der_match. auto.
         * symmetry in H. apply max_pref_fn_splits in H. injection H. intros. contradiction.
   Qed.
@@ -415,7 +368,7 @@ Module LemmasFn (Import ST : state.T).
   
    Theorem re_max_pref_correct__None : forall(code : String) (e : regex),
       re_no_max_pref code e
-      <-> None = max_pref_fn code (init_state e).
+      <-> None = max_pref_fn code (init_index (length code)) (init_state e).
    Proof.
      
      induction code.
@@ -436,23 +389,26 @@ Module LemmasFn (Import ST : state.T).
        - simpl. repeat dm.
          + rewrite mpref_cons in E.
            symmetry in E.
-           assert(E1 := E).
+           assert(E2 := E).
            apply max_pref_fn_splits in E. injection E. intros. clear E.
-           apply max_pref_matches in E1.
-           inv H. specialize (H1 (a :: p0)). destruct H1; auto.
+           rewrite incr_inv_decr in *. apply max_pref_matches in E2.
+           inv H. specialize (H1 (a :: p1)). destruct H1; auto.
            apply pref_def. exists s. auto.
-         + clear H. symmetry in E. rewrite mpref_dt in E. apply IHcode in E.
+         + clear H. symmetry in E. rewrite mpref_dt in E.
+           rewrite decr_inv_S in *. apply IHcode in E.
            inv E. specialize (H1 []). destruct H1. apply nil_is_prefix.
            rewrite accepts_nil in E0. rewrite accepts_transition in E0.
            symmetry in E0. apply accepts_matches in E0. apply der_match. auto.
-         + symmetry in E. rewrite mpref_dt in E. apply IHcode in E.
+         + symmetry in E. rewrite mpref_dt in E.
+           rewrite decr_inv_S in *. apply IHcode in E.
            inv E. specialize (H1 []). destruct H1. apply nil_is_prefix.
            inv H. specialize (H1 []). destruct H1.
            * apply nil_is_prefix.
            * rewrite accepts_nil in E1. symmetry in E1. apply accepts_matches in E1.
              auto.
        - simpl in H. repeat dm; try(discriminate).
-         clear H. rewrite mpref_dt in E. symmetry in E. apply IHcode in E.
+         clear H. rewrite mpref_dt in E. symmetry in E.
+         rewrite decr_inv_S in *. apply IHcode in E.
          inv E. apply re_MP0. intros. intros C. inv H. destruct H0.
          destruct cand.
          + rewrite false_not_true in E1. destruct E1.
@@ -462,11 +418,29 @@ Module LemmasFn (Import ST : state.T).
            * apply pref_def. eexists. eauto.
            * apply der_match. auto.
      } 
-   Qed.          
+   Qed.
+
+   Theorem index_closure : forall code p q qi e,
+       Some (p, q, qi)
+       = max_pref_fn code (init_index (length code)) (init_state e)
+       ->  qi = (init_index (length q)).
+   Proof.
+     induction code; intros.
+     - sis. repeat dm.
+       + repeat inj_all. sis. auto.
+       + discriminate.
+     - sis. repeat dm.
+       + rewrite decr_inv_S in *. symmetry in E. rewrite mpref_dt in *. apply IHcode in E.
+         repeat inj_all. auto.
+       + repeat inj_all. apply decr_inv_S.
+       + repeat inj_all. sis. auto.
+       + discriminate.
+   Qed.
   
   Theorem re_max_pref_correct__Some : forall(code p : String) (e : regex),
       re_max_pref code e p
-      <-> exists(q : String), Some (p, q) = max_pref_fn code (init_state e).
+      <-> exists(q : String), Some (p, q, (init_index (length q)))
+                       = max_pref_fn code (init_index (length code)) (init_state e).
   Proof.
     induction code.
     {
@@ -497,7 +471,7 @@ Module LemmasFn (Import ST : state.T).
           assert (A1 : p = []).
           {
             simpl in H. dm.
-            - injection H. intros I1 I2. apply I2.
+            - injection H. intros. auto. 
             - discriminate.
           }
           rewrite A0. rewrite A1. left. omega.
@@ -507,9 +481,15 @@ Module LemmasFn (Import ST : state.T).
       - destruct p.
         + exists (a :: code). inv H. simpl.
           dm.
-          * destruct p. symmetry in E.
+          * destruct p. destruct p. symmetry in E.
             rewrite mpref_dt in E.
-            assert (Ae : exists q, Some (p, q) = max_pref_fn code (init_state (derivative a e))).
+            rewrite decr_inv_S in *.
+            assert( i = init_index (length s)).
+            { eapply index_closure in E. auto. }
+            rewrite H in *. clear H.
+            assert (Ae : exists q, Some (p, q, init_index (length q))
+                              = max_pref_fn code (init_index (length code))
+                                            (init_state (derivative a e))).
             { exists s. apply E. }
             apply IHcode in Ae. inv Ae.
             assert (Ap : a :: p ++_= a :: code).
@@ -523,7 +503,7 @@ Module LemmasFn (Import ST : state.T).
               - simpl in E. dm.
                 + discriminate.
               - simpl in E. dm.
-                + destruct p. discriminate.
+                + destruct p. dm. discriminate.
                 + dm.
                   * discriminate.
                   * dm.
@@ -536,8 +516,14 @@ Module LemmasFn (Import ST : state.T).
           assert (Ap : p ++_= code).
           { apply pref_def. exists x. apply I1. }
           simpl. dm; symmetry in E.
-          * destruct p0.
-            assert (Ae : exists q, Some (p0, q) = max_pref_fn code (init_state (derivative a e))).
+          * destruct p0. destruct p0.
+            rewrite decr_inv_S in *.
+            assert(i = init_index (length s)). symmetry in E. rewrite mpref_cons in E.
+            { symmetry in E. erewrite <- index_incr_cons in *. apply index_closure in E. auto. }
+            rewrite H in *. clear H.
+            assert (Ae : exists q, Some (p0, q, init_index (length q))
+                              = max_pref_fn code (init_index (length code))
+                                           (init_state (derivative a e))).
             { exists s. symmetry in E. rewrite mpref_dt in E. auto. }
             apply IHcode in Ae. inv Ae. inv H1. destruct H5. apply max_pref_fn_splits in E.
             (* Want to show p = p0 *)
@@ -567,7 +553,8 @@ Module LemmasFn (Import ST : state.T).
             -- rewrite A. rewrite A in E. apply app_inv_head in E. rewrite E. reflexivity.
             -- apply As.
             -- apply Ap.
-          * rewrite mpref_dt in E. apply re_max_pref_correct__None in E. inv E.
+          * rewrite mpref_dt in E. rewrite decr_inv_S in *.
+            apply re_max_pref_correct__None in E. inv E.
             assert (A0 : p = []).
             {
               assert (A1 : p ++_= p ++ x).
@@ -586,11 +573,11 @@ Module LemmasFn (Import ST : state.T).
         + intros cand Hpref. destruct p.
           * simpl in H.
             dm.
-            -- destruct p. discriminate.
+            -- destruct p. destruct p. discriminate.
             -- dm.
                ++ discriminate.
                ++ dm.
-                  ** symmetry in E. rewrite mpref_dt in E.
+                  ** symmetry in E. rewrite mpref_dt in E. rewrite decr_inv_S in *.
                      apply re_max_pref_correct__None in E. inv E. destruct cand.
                      { left. omega. }
                      {
@@ -604,19 +591,25 @@ Module LemmasFn (Import ST : state.T).
                   ** discriminate.
           * simpl in H.
             dmh; symmetry in E.
-            -- destruct p0. injection H. intros I1 I2 I3.
-               rewrite mpref_dt in E.
-               assert (Ae : exists q, Some (p0, q) = max_pref_fn code (init_state (derivative a e))).
+            -- destruct p0. destruct p0. injection H. intros I1 I2 I3 I4.
+               rewrite decr_inv_S in *. rewrite mpref_dt in E.
+               assert(i = init_index (length s0)).
+               { repeat inj_all. auto. }
+               rewrite H0 in *. clear H0.
+               assert (Ae : exists q, Some (p0, q, init_index (length q))
+                                 = max_pref_fn code (init_index (length code))
+                                               (init_state (derivative a e))).
                { exists s0. apply E. }
                apply IHcode in Ae. inv Ae. destruct cand.
                ++ left. simpl. omega.
-               ++ inv Hpref. destruct H0. injection H0. intros I1 I2. subst s.
+               ++ inv Hpref. destruct H0. injection H0. intros. subst s.
                   assert (Apref : cand ++_= code).
-                  { apply pref_def. exists x. apply I1. }
+                  { apply pref_def. exists x. auto. }
                   apply H3 in Apref. destruct Apref.
                   ** left. simpl. omega.
-                  ** right. intros C. destruct H4. apply der_match. auto.
-            -- rewrite mpref_dt in E. apply re_max_pref_correct__None in E. inv E.
+                  ** right. intros C. destruct H5. apply der_match. auto.
+            -- rewrite mpref_dt in E. rewrite decr_inv_S in *.
+               apply re_max_pref_correct__None in E. inv E.
                assert (A0 : accepting (transition a (init_state e)) = true).
                {
                  repeat dm;
@@ -632,10 +625,10 @@ Module LemmasFn (Import ST : state.T).
     }
   Qed.
 
-  Lemma no_tokens_suffix_self : forall rus code rest Ha,
-      lex' rus code Ha = ([], rest) -> code = rest.
+  Lemma no_tokens_suffix_self : forall rus code rest i Hindex Ha,
+      lex' rus code i Hindex Ha = ([], rest) -> code = rest.
   Proof.
-    intros rus code rest Ha H.
+    intros rus code rest i Hindex Ha H.
     apply lex'_cases in H. destruct H.
     symmetry. apply H.
   Qed.
@@ -648,12 +641,15 @@ Module LemmasFn (Import ST : state.T).
     apply H0 in H1. contradiction.
   Qed.
 
-  Lemma max_pref_fn_Some_or_None : forall code fsm,
-      (exists p q, Some (p, q) = max_pref_fn code fsm)
-      \/ None = max_pref_fn code fsm.
+  Lemma max_pref_fn_Some_or_None : forall code e,
+      (exists p q, Some (p, q, init_index (length q))
+      = max_pref_fn code (init_index (length code)) (init_state e))
+      \/ None = max_pref_fn code (init_index (length code)) (init_state e).
   Proof.
-    intros code fsm. destruct (max_pref_fn code fsm).
-    - left. destruct p. exists p. exists s. reflexivity.
+    intros code e.
+    destruct (max_pref_fn code (init_index (length code)) (init_state e)) eqn:E.
+    - left. destruct p. destruct p. exists p. exists s. symmetry in E.  apply index_closure in E.
+      subst. reflexivity.
     - right. reflexivity.
   Qed.
 
@@ -663,7 +659,7 @@ Module LemmasFn (Import ST : state.T).
   Proof.
     intros code r. 
     assert(L := max_pref_fn_Some_or_None).
-    specialize (L code). specialize (L (init_state r)). destruct L.
+    specialize (L code). specialize (L r). destruct L.
     - left. destruct H as [p]. apply re_max_pref_correct__Some in H.
       eexists; eauto.
     - right. apply re_max_pref_correct__None in H. auto.
@@ -790,8 +786,8 @@ Module LemmasFn (Import ST : state.T).
       try(auto).
   Qed.
 
-  Lemma all_mprefs_nil : forall label p ps suffix rs r,
-      max_of_prefs (max_prefs [] (r :: rs)) <> (label, Some (p :: ps, suffix)).
+  Lemma all_mprefs_nil : forall label p ps suffix i i' rs r,
+      max_of_prefs (max_prefs [] i (r :: rs)) <> (label, Some (p :: ps, suffix, i')).
   Proof.
     intros label p ps suffix. induction rs; intros.
     - intro C. simpl in *. unfold extract_fsm_for_max in *. unfold longer_pref in *. simpl.
@@ -817,9 +813,61 @@ Module LemmasFn (Import ST : state.T).
     intros ps p. simpl. reflexivity.
   Qed.
 
+  Lemma exists_rus_of_mpref_gen : forall rus code l px suffix i,
+      max_of_prefs (max_prefs code (init_index (length code)) rus)
+      = (l, Some (px, suffix, i))
+      -> (exists r, In (l, r) rus
+              /\ max_pref_fn code (init_index (length code)) r
+                = Some (px, suffix, i)).
+  Proof.
+    induction rus; intros.
+    {
+      simpl in H. discriminate.
+    }
+    {
+      unfold max_prefs in H.
+      repeat first [rewrite map_cons in H | rewrite map_app in H].
+      symmetry in H. apply max_first_or_rest in H. destruct H.
+      - destruct a. simpl in H. injection H; intros; subst.
+        exists s. split.
+        * left. auto.
+        * auto.
+      - symmetry in H. apply IHrus in H. destruct H as [r]. destruct H.
+        exists r. split.
+        + right. apply H.
+        + apply H0.
+    }
+  Qed.
+  
+  Lemma exists_rus_of_mpref : forall rus code l px suffix i,
+      max_of_prefs (max_prefs code (init_index (length code)) (map init_srule rus))
+      = (l, Some (px, suffix, i))
+      -> (exists r, In (l, r) rus
+              /\ max_pref_fn code (init_index (length code)) (init_state r)
+                                  = Some (px, suffix, i)).
+  Proof.
+    induction rus; intros.
+    {
+      simpl in H. discriminate.
+    }
+    {
+      unfold max_prefs in H.
+      repeat first [rewrite map_cons in H | rewrite map_app in H].
+      symmetry in H. apply max_first_or_rest in H. destruct H.
+      - destruct a. simpl in H. injection H; intros; subst.
+        exists r. split.
+        * left. auto.
+        * auto.
+      - symmetry in H. apply IHrus in H. destruct H as [r]. destruct H.
+        exists r. split.
+        + right. apply H.
+        + apply H0.
+    }
+  Qed.
   
   Lemma nil_mpref_nil_or_no_pref : forall rus code s l l1 r,
-      max_of_prefs (max_prefs code (map init_srule rus)) = (l1, Some ([], s))
+      max_of_prefs (max_prefs code (init_index (length code)) (map init_srule rus))
+                    = (l1, Some ([], s, init_index (length s)))
       -> In (l, r) rus
       -> re_max_pref code r [] \/ re_no_max_pref code r.
   Proof.
@@ -833,28 +881,25 @@ Module LemmasFn (Import ST : state.T).
         assert(L := (part_around_in _ rus (l, r)) Hin).
         destruct L as (rus1 & rus2 & L). subst rus. clear Hin.
         rewrite map_app in Hmax. rewrite map_cons in Hmax. simpl in Hmax.
-        unfold max_prefs in Hmax. rewrite map_app in Hmax. rewrite map_cons in Hmax. simpl in Hmax.
+        unfold max_prefs in Hmax. rewrite map_app in Hmax. rewrite map_cons in Hmax.
+        simpl in Hmax.
         rewrite H in Hmax. rewrite mpref_app_dist in Hmax. rewrite mpref_cons_longer in Hmax.
         simpl in Hmax. unfold longer_pref in Hmax.
         (* 32 subgoals, 7 subproofs ! *)
         repeat dmh; subst;
-          try (discriminate);
-          try(injection Hmax; intros I1 I2 I3; subst p0;
-              destruct p2; [discriminate | simpl in E5; discriminate]);
-          try(injection E2; intros; subst; discriminate);
-          try(rewrite Hmax in E1; discriminate).
-        * injection E2; intros; injection Hmax; intros; subst;
-            rewrite E11 in E5; simpl in E5; discriminate.
-        * injection E2; intros; injection Hmax; intros; subst;
-            destruct (length p0); simpl in E6; rewrite Nat.ltb_lt in E6; omega.
-        * rewrite Hmax in E1. injection E1; intros; subst. simpl in E7; discriminate.
+          try (repeat inj_all; discriminate).
+        * repeat inj_all. rewrite Nat.eqb_eq in *. sis. omega.
+        * repeat inj_all. rewrite false_not_true in *. destruct E8.
+          rewrite Nat.ltb_lt. sis. omega.
+          
     - right. apply H.
   Qed.
    
 
   
   Lemma no_mpref_no_pref : forall rus code l l1 r,
-      max_of_prefs (max_prefs code (map init_srule rus)) = (l1, None)
+      max_of_prefs (max_prefs code (init_index (length code)) (map init_srule rus))
+      = (l1, None)
       -> In (l, r) rus
       -> re_no_max_pref code r.
   Proof.
@@ -875,21 +920,33 @@ Module LemmasFn (Import ST : state.T).
     - apply H.
   Qed.
   
-
+  Lemma index_closure_mprefs : forall code rus l0 px suf x,
+    max_of_prefs (max_prefs code (init_index (length code)) (map init_srule rus))
+    = (l0, Some (px, suf, x))
+    -> x = init_index (length suf).
+  Proof.
+    intros. apply exists_rus_of_mpref in H. destruct H. destruct H.
+    eapply index_closure; eauto.
+  Qed.
   
-  Lemma no_tokens_no_pref : forall code rest rus l r Ha,
-      lex' (map init_srule rus) code Ha = ([], rest)
+  Lemma no_tokens_no_pref : forall code rest rus l r i Hindex Ha,
+      lex' (map init_srule rus) code i Hindex Ha = ([], rest)
       -> In (l, r) rus
       -> re_max_pref code r [] \/ re_no_max_pref code r.
   Proof.
-    intros code rest rus l r Ha Hlex Hin.
+    intros code rest rus l r i Hindex Ha Hlex Hin.
     apply lex'_cases in Hlex. destruct Hlex.
-    destruct H0; destruct (max_of_prefs (max_prefs code (map init_srule rus))) eqn:E0;
-      simpl in H0; [| destruct H0 as (suf & H0)]; rewrite H0 in E0.
-    - apply no_mpref_no_pref with (l := l) (r := r) in E0.
+    destruct H0; destruct (max_of_prefs (max_prefs code i (map init_srule rus))) eqn:E0;
+      simpl in H0; [| destruct H0 as (suf & H0)]. 
+    - rewrite H0 in E0. rewrite Hindex in *.
+      apply no_mpref_no_pref with (l := l) (r := r) in E0.
       + right. apply E0.
       + apply Hin.
-    - apply nil_mpref_nil_or_no_pref with (l := l) (r := r) in E0.
+    - destruct H0. rewrite H0 in E0. rewrite Hindex in *.
+      assert(x = init_index (length suf)).
+      { eapply index_closure_mprefs; eauto. }
+      rewrite H1 in *. clear H1.
+      apply nil_mpref_nil_or_no_pref with (l := l) (r := r) in E0.
       + apply E0.
       + apply Hin.
   Qed.
@@ -911,16 +968,16 @@ Module LemmasFn (Import ST : state.T).
     apply Aeq. apply Hp. apply Hp'.
   Qed.
 
-  Lemma max_pref_longer : forall xs l p s l' p' s' code,
-      max_of_prefs xs = (l, Some(p, s))
-      -> In (l', Some(p', s')) xs
-      -> (l', Some(p', s')) <> (l, Some(p, s))
+  Lemma max_pref_longer : forall xs l p s i l' p' s' i' code,
+      max_of_prefs xs = (l, Some(p, s, i))
+      -> In (l', Some(p', s', i')) xs
+      -> (l', Some(p', s', i')) <> (l, Some(p, s, i))
       -> p ++_= code
       -> p' ++_= code
-      -> longer_pref (l, Some(p, s)) (l', Some(p', s')) = (l, Some(p, s)).
+      -> longer_pref (l, Some(p, s, i)) (l', Some(p', s', i')) = (l, Some(p, s, i)).
   Proof.
-    intros xs l p s l' p' s' code Hmax Hin Hneq Hpref Hpref'.
-    assert(Apart : exists xs1 xs2, xs = xs1 ++ ((l', Some(p', s')) :: xs2)).
+    intros xs l p s i l' p' s' i' code Hmax Hin Hneq Hpref Hpref'.
+    assert(Apart : exists xs1 xs2, xs = xs1 ++ ((l', Some(p', s', i')) :: xs2)).
     { apply part_around_in. apply Hin.  }
     destruct Apart as (xs1 & xs2 & Apart).
     rewrite Apart in *.
@@ -963,42 +1020,21 @@ Module LemmasFn (Import ST : state.T).
         * simpl. simpl in H5. rewrite H5. auto.
   Qed.
 
-  Lemma exists_rus_of_mpref : forall rus code l ph pt suffix,
-      max_of_prefs (max_prefs code (map init_srule rus)) = (l, Some (ph :: pt, suffix))
-      -> (exists r, In (l, r) rus
-              /\ max_pref_fn code (init_state r) = Some (ph :: pt, suffix)).
-  Proof.
-    induction rus; intros.
-    {
-      simpl in H. discriminate.
-    }
-    {
-      unfold max_prefs in H.
-      repeat first [rewrite map_cons in H | rewrite map_app in H].
-      symmetry in H. apply max_first_or_rest in H. destruct H.
-      - destruct a. simpl in H. injection H; intros; subst.
-        exists r. split.
-        * left. auto.
-        * auto.
-      - symmetry in H. apply IHrus in H. destruct H as [r]. destruct H.
-        exists r. split.
-        + right. apply H.
-        + apply H0.
-    }
-  Qed.
 
   Lemma first_token_mpref : forall rus code l ph pt suffix,
-      max_of_prefs (max_prefs code (map init_srule rus)) = (l, Some (ph :: pt, suffix))
+      max_of_prefs (max_prefs code (init_index (length code)) (map init_srule rus))
+      = (l, Some (ph :: pt, suffix, init_index (length suffix)))
       -> rules_is_function rus
       -> first_token code rus (l, ph :: pt).
   Proof.
     intros rus code l ph pt suffix H Hfunc.
-    assert(Aex := exists_rus_of_mpref rus code l ph pt suffix H).
+    assert(Aex := exists_rus_of_mpref rus code l (ph :: pt) suffix _  H).
     destruct Aex as [r]. destruct H0 as (Hin & Hmpref_fn).
     assert(Hmpref : re_max_pref code r (ph :: pt)).
     {
       symmetry in Hmpref_fn.
-      assert(exists q, Some (ph :: pt, q) = max_pref_fn code (init_state r)).
+      assert(exists q, Some (ph :: pt, q, init_index (length q))
+                  = max_pref_fn code (init_index (length code)) (init_state r)).
       { eexists; eauto. }
       apply re_max_pref_correct__Some in H0. auto.
     }
@@ -1008,17 +1044,18 @@ Module LemmasFn (Import ST : state.T).
     - apply Hmpref.
     - intros l0 r0 p0 Hlen Hmpref'. intros C.
       apply re_max_pref_correct__Some with (e := r0) in Hmpref'. destruct Hmpref'.
-      assert(Ain : In (l0, max_pref_fn code (init_state r0))
-                      (max_prefs code (map init_srule rus))).
+      assert(Ain : In (l0, max_pref_fn code (init_index (length code)) (init_state r0))
+                      (max_prefs code (init_index (length code)) (map init_srule rus))).
       {
         apply part_around_in in C. destruct C as (rus1 & rus2 & C). rewrite C.
         unfold max_prefs. repeat rewrite map_app. repeat rewrite map_cons. simpl.
         apply in_or_app. right. simpl. left. reflexivity.
       }
-      assert(Aneq : (l0, max_pref_fn code (init_state r0)) <> (l, Some (ph :: pt, suffix))).
+      assert(Aneq : (l0, max_pref_fn code (init_index (length code)) (init_state r0))
+                    <> (l, Some (ph :: pt, suffix, init_index (length suffix)))).
       { rewrite <- H0. intros C1. injection C1; intros; subst. omega. }
       apply max_pref_longer
-        with (l' := l0) (p' := p0) (s' := x) (code := code)
+        with (l' := l0) (p' := p0) (s' := x) (code := code) (i' := init_index (length x))
         in H.
       + rewrite <- H0 in *. unfold longer_pref in H. repeat dmh.
         * eqb_eq_all. omega.
@@ -1027,11 +1064,13 @@ Module LemmasFn (Import ST : state.T).
       + rewrite <- H0 in Ain. apply Ain.
       + rewrite <- H0 in Aneq. apply Aneq.
       + inv Hmpref. apply H1.
-      + assert(A : exists q, Some (p0, q) = max_pref_fn code (init_state r0)).
+      + assert(A : exists q, Some (p0, q, init_index (length q))
+                        = max_pref_fn code (init_index (length code)) (init_state r0)).
         { exists x. apply H0. }
         apply re_max_pref_correct__Some in A. inv A. apply H1.
     - intros r0 l0 Hearly Hin0 Hmpref0.
-      assert(Hmpref_fn0 : max_pref_fn code (init_state r0) = Some (ph :: pt, suffix)).
+      assert(Hmpref_fn0 : max_pref_fn code (init_index (length code)) (init_state r0)
+                          = Some (ph :: pt, suffix, init_index (length suffix))).
       {
         apply re_max_pref_correct__Some with (e := r0) in Hmpref0.
         destruct Hmpref0 as (x & Hmpref_fn0).
@@ -1075,8 +1114,9 @@ Module LemmasFn (Import ST : state.T).
       destruct Alt as (x & y & H1). destruct H1. destruct H2.
       clear H0 Heq Heq'.
       rewrite H3 in *.
-      assert(A0 : max_of_prefs (map (extract_fsm_for_max code) (map init_srule rus1')) <>
-                  (l, Some (ph :: pt, suffix))).
+      assert(A0 : max_of_prefs (map (extract_fsm_for_max code (init_index (length code)))
+                                    (map init_srule rus1'))
+                                <>  (l, Some (ph :: pt, suffix, init_index (length suffix)))).
       {
         intros C. apply exists_rus_of_mpref in C.
         destruct C as (r' & C). destruct C as (C1 & C2).
@@ -1099,18 +1139,18 @@ Module LemmasFn (Import ST : state.T).
           try(omega); try(contradiction); try(discriminate).
   Qed.
 
-  Lemma lex'_splits : forall ts code rest rus Ha,
-      lex' (map init_srule rus) code Ha = (ts, rest)
+  Lemma lex'_splits : forall ts code rest rus i Hindex Ha,
+      lex' (map init_srule rus) code i Hindex Ha = (ts, rest)
       -> code = (concat (map snd ts)) ++ rest.
   Proof.
-    induction ts; intros code rest rus Ha H.
+    induction ts; intros code rest rus i Hindex Ha H.
     {
       simpl. apply no_tokens_suffix_self in H. auto.
     }
     {
       destruct a. apply lex'_cases in H.
-      destruct H as (h & t & H). destruct H as (s & Heq & H).
-      destruct H. apply IHts in H.
+      destruct H as (h & t & H). destruct H as (s & i' & Heq & H).
+      destruct H. apply IHts in H. rewrite Hindex in *.
       apply exists_rus_of_mpref in Heq. destruct Heq. destruct H1.
       symmetry in H2. apply max_pref_fn_splits in H2.
       subst. simpl.
