Verbatim/regex.v
@@ -109,105 +109,106 @@ Module DefsFn (Ty : SIGMA).
           * right. apply IHyss. apply H.
     Qed.
 
-    End Strings.
+  End Strings.
 
-    Module Export Regexes.
 
-      Inductive regex : Type :=
-      | EmptySet
-      | EmptyStr
-      | Char (t : Sigma)
-      | App (r1 r2 : regex)
-      | Union (r1 r2 : regex)
-      | Star (r : regex).
+  Module Export Regexes.
 
-      Lemma regex_dec : forall r r' : regex, {r = r'} + {r <> r'}.
-      Proof. decide equality. Qed.
+    Inductive regex : Type :=
+    | EmptySet
+    | EmptyStr
+    | Char (t : Sigma)
+    | App (r1 r2 : regex)
+    | Union (r1 r2 : regex)
+    | Star (r : regex).
 
-      (** * *Should rename to re_equal *)
-      Fixpoint regex_eq (r1 r2 : regex) : bool :=
-        match r1, r2 with
-        | EmptyStr, EmptyStr => true
-        | EmptySet, EmptySet => true
-        | Char a, Char b => if (Ty.Sigma_dec a b) then true else false
-        | App x1 y1, App x2 y2 => andb (regex_eq x1 x2) (regex_eq y1 y2)
-        | Union x1 y1, Union x2 y2 => andb (regex_eq x1 x2) (regex_eq y1 y2)
-        | Star a, Star b => regex_eq a b
-        | _, _ => false
-        end.
+    Lemma regex_dec : forall r r' : regex, {r = r'} + {r <> r'}.
+    Proof. decide equality. Qed.
 
-      Lemma regex_eq_correct : forall r1 r2,
-          r1 = r2 <-> regex_eq r1 r2 = true.
-      Proof.
-        induction r1; intros r2; split; intros H; subst; try(auto);
-          try(unfold regex_eq in H; repeat dmh; subst; auto; discriminate).
-        - simpl. dmg; [reflexivity | contradiction].
-        - assert(A1 : regex_eq r1_1 r1_1 = true). apply IHr1_1; reflexivity.
-          assert(A2 : regex_eq r1_2 r1_2 = true). apply IHr1_2; reflexivity.
-          simpl. rewrite A1. rewrite A2. auto.
-        - destruct r2; simpl in H; try(discriminate).
-          destruct (regex_eq r1_1 r2_1) eqn:E1; destruct (regex_eq r1_2 r2_2) eqn:E2; try(discriminate).
-          apply IHr1_1 in E1. apply IHr1_2 in E2. subst. reflexivity.
-        - assert(A1 : regex_eq r1_1 r1_1 = true). apply IHr1_1; reflexivity.
-          assert(A2 : regex_eq r1_2 r1_2 = true). apply IHr1_2; reflexivity.
-          simpl. rewrite A1. rewrite A2. auto.
-        - destruct r2; simpl in H; try(discriminate).
-          destruct (regex_eq r1_1 r2_1) eqn:E1; destruct (regex_eq r1_2 r2_2) eqn:E2; try(discriminate).
-          apply IHr1_1 in E1. apply IHr1_2 in E2. subst. reflexivity.
-        - assert(A : regex_eq r1 r1 = true). apply IHr1; reflexivity.
-          simpl. apply A.
-        - destruct r2; simpl in H; try(discriminate). apply IHr1 in H. subst; reflexivity.
-      Qed.
+    (** * *Should rename to re_equal *)
+    Fixpoint regex_eq (r1 r2 : regex) : bool :=
+      match r1, r2 with
+      | EmptyStr, EmptyStr => true
+      | EmptySet, EmptySet => true
+      | Char a, Char b => if (Ty.Sigma_dec a b) then true else false
+      | App x1 y1, App x2 y2 => andb (regex_eq x1 x2) (regex_eq y1 y2)
+      | Union x1 y1, Union x2 y2 => andb (regex_eq x1 x2) (regex_eq y1 y2)
+      | Star a, Star b => regex_eq a b
+      | _, _ => false
+      end.
 
-      Lemma regex_eq_refl : forall e, regex_eq e e = true.
-        intros. induction e; auto.
-        - simpl. dm.
-        - simpl. apply Bool.andb_true_iff. split; auto.
-        - simpl. apply Bool.andb_true_iff. split; auto.
-      Qed.
+    Lemma regex_eq_correct : forall r1 r2,
+        r1 = r2 <-> regex_eq r1 r2 = true.
+    Proof.
+      induction r1; intros r2; split; intros H; subst; try(auto);
+        try(unfold regex_eq in H; repeat dmh; subst; auto; discriminate).
+      - simpl. dmg; [reflexivity | contradiction].
+      - assert(A1 : regex_eq r1_1 r1_1 = true). apply IHr1_1; reflexivity.
+        assert(A2 : regex_eq r1_2 r1_2 = true). apply IHr1_2; reflexivity.
+        simpl. rewrite A1. rewrite A2. auto.
+      - destruct r2; simpl in H; try(discriminate).
+        destruct (regex_eq r1_1 r2_1) eqn:E1; destruct (regex_eq r1_2 r2_2) eqn:E2; try(discriminate).
+        apply IHr1_1 in E1. apply IHr1_2 in E2. subst. reflexivity.
+      - assert(A1 : regex_eq r1_1 r1_1 = true). apply IHr1_1; reflexivity.
+        assert(A2 : regex_eq r1_2 r1_2 = true). apply IHr1_2; reflexivity.
+        simpl. rewrite A1. rewrite A2. auto.
+      - destruct r2; simpl in H; try(discriminate).
+        destruct (regex_eq r1_1 r2_1) eqn:E1; destruct (regex_eq r1_2 r2_2) eqn:E2; try(discriminate).
+        apply IHr1_1 in E1. apply IHr1_2 in E2. subst. reflexivity.
+      - assert(A : regex_eq r1 r1 = true). apply IHr1; reflexivity.
+        simpl. apply A.
+      - destruct r2; simpl in H; try(discriminate). apply IHr1 in H. subst; reflexivity.
+    Qed.
 
-      Fixpoint nullable' (r : regex) : bool:=
-        match r with
-        | EmptySet => false
-        | EmptyStr => true
-        | Char _ => false
-        | App r1 r2 => andb (nullable' r1) (nullable' r2)
-        | Union r1 r2 => orb (nullable' r1) (nullable' r2)
-        | Star _ => true
-        end.
+    Lemma regex_eq_refl : forall e, regex_eq e e = true.
+      intros. induction e; auto.
+      - simpl. dm.
+      - simpl. apply Bool.andb_true_iff. split; auto.
+      - simpl. apply Bool.andb_true_iff. split; auto.
+    Qed.
 
-      Fixpoint nullable (r : regex) : bool:=
-        match r with
-        | EmptySet => false
-        | EmptyStr => true
-        | Char _ => false
-        | App r1 r2 => if negb (nullable r2) (* short circuit and *)
-                      then false
+    Fixpoint nullable' (r : regex) : bool:=
+      match r with
+      | EmptySet => false
+      | EmptyStr => true
+      | Char _ => false
+      | App r1 r2 => andb (nullable' r1) (nullable' r2)
+      | Union r1 r2 => orb (nullable' r1) (nullable' r2)
+      | Star _ => true
+      end.
+
+    Fixpoint nullable (r : regex) : bool:=
+      match r with
+      | EmptySet => false
+      | EmptyStr => true
+      | Char _ => false
+      | App r1 r2 => if negb (nullable r2) (* short circuit and *)
+                    then false
+                    else (nullable r1)
+      | Union r1 r2 => if (nullable r2)    (* short circuit or *)
+                      then true
                       else (nullable r1)
-        | Union r1 r2 => if (nullable r2)    (* short circuit or *)
-                        then true
-                        else (nullable r1)
-        | Star _ => true
-        end.
-      
-      Fixpoint derivative (a : Sigma) (r : regex) :=
-        match r with
-        | EmptySet => EmptySet
-        | EmptyStr => EmptySet
-        | Char x => if Ty.Sigma_dec x a then EmptyStr else EmptySet
-        | App r1 r2 => if (nullable r1) then Union (App (derivative a r1) r2) (derivative a r2)
-                      else (App (derivative a r1) r2)
-        | Union r1 r2 => Union (derivative a r1) (derivative a r2)
-        | Star r => App (derivative a r) (Star r)
-        end.
+      | Star _ => true
+      end.
+    
+    Fixpoint derivative (a : Sigma) (r : regex) :=
+      match r with
+      | EmptySet => EmptySet
+      | EmptyStr => EmptySet
+      | Char x => if Ty.Sigma_dec x a then EmptyStr else EmptySet
+      | App r1 r2 => if (nullable r1) then Union (App (derivative a r1) r2) (derivative a r2)
+                    else (App (derivative a r1) r2)
+      | Union r1 r2 => Union (derivative a r1) (derivative a r2)
+      | Star r => App (derivative a r) (Star r)
+      end.
 
-      Fixpoint derivative_list (bs : list Sigma) (e : regex) :=
-        match bs with
-        | [] => e
-        | c :: cs => derivative_list cs (derivative c e)
-        end.
+    Fixpoint derivative_list (bs : list Sigma) (e : regex) :=
+      match bs with
+      | [] => e
+      | c :: cs => derivative_list cs (derivative c e)
+      end.
 
-      Fixpoint re_compare (e1 e2 : regex) : comparison :=
+    Fixpoint re_compare (e1 e2 : regex) : comparison :=
       match e1, e2 with
       | EmptyStr, EmptyStr => Eq
       | EmptyStr, _ => Lt
@@ -235,368 +236,368 @@ Module DefsFn (Ty : SIGMA).
         end
       end.
 
-      Lemma re_compare_eq : forall x y : regex, re_compare x y = Eq <-> x = y.
-      Proof.
-        induction x; destruct y; split;
-          try(reflexivity);
-          try(simpl; intros; discriminate).
-        - simpl. intros. apply compareT_eq in H. subst. auto.
-        - simpl. intros. injection H; intros; subst. apply compareT_eq. auto.
-        - intros. specialize (IHx1 y1). specialize (IHx2 y2). simpl in H.
-          destruct (re_compare x1 y1) eqn:E; try(discriminate).
-          destruct IHx1. destruct H0. auto. destruct (re_compare x2 y2); try(discriminate).
-          destruct IHx2. destruct H0; auto.
-        - intros. injection H. intros; subst. simpl.
-          destruct (regex_eq y1 y1) eqn:E.
-          + apply regex_eq_correct in E. apply IHx1 in E. rewrite E.
-            destruct (regex_eq y2 y2) eqn:E1.
-            * apply regex_eq_correct in E1. apply IHx2 in E1. auto.
-            * apply false_not_true in E1. destruct E1. apply regex_eq_correct. auto.
-          + apply false_not_true in E. destruct E. apply regex_eq_correct. auto.
-        - intros. specialize (IHx1 y1). specialize (IHx2 y2). simpl in H.
-          destruct (re_compare x1 y1) eqn:E; try(discriminate).
-          destruct IHx1. destruct H0. auto. destruct (re_compare x2 y2); try(discriminate).
-          destruct IHx2. destruct H0; auto.
-        - intros. injection H. intros; subst. simpl.
-          destruct (regex_eq y1 y1) eqn:E.
-          + apply regex_eq_correct in E. apply IHx1 in E. rewrite E.
-            destruct (regex_eq y2 y2) eqn:E1.
-            * apply regex_eq_correct in E1. apply IHx2 in E1. auto.
-            * apply false_not_true in E1. destruct E1. apply regex_eq_correct. auto.
-          + apply false_not_true in E. destruct E. apply regex_eq_correct. auto.
-        - intros. specialize (IHx y). simpl in H. apply IHx in H. subst. auto.
-        - intros. injection H. intros. subst. simpl. apply IHx. auto.
-      Qed.
+    Lemma re_compare_eq : forall x y : regex, re_compare x y = Eq <-> x = y.
+    Proof.
+      induction x; destruct y; split;
+        try(reflexivity);
+        try(simpl; intros; discriminate).
+      - simpl. intros. apply compareT_eq in H. subst. auto.
+      - simpl. intros. injection H; intros; subst. apply compareT_eq. auto.
+      - intros. specialize (IHx1 y1). specialize (IHx2 y2). simpl in H.
+        destruct (re_compare x1 y1) eqn:E; try(discriminate).
+        destruct IHx1. destruct H0. auto. destruct (re_compare x2 y2); try(discriminate).
+        destruct IHx2. destruct H0; auto.
+      - intros. injection H. intros; subst. simpl.
+        destruct (regex_eq y1 y1) eqn:E.
+        + apply regex_eq_correct in E. apply IHx1 in E. rewrite E.
+          destruct (regex_eq y2 y2) eqn:E1.
+          * apply regex_eq_correct in E1. apply IHx2 in E1. auto.
+          * apply false_not_true in E1. destruct E1. apply regex_eq_correct. auto.
+        + apply false_not_true in E. destruct E. apply regex_eq_correct. auto.
+      - intros. specialize (IHx1 y1). specialize (IHx2 y2). simpl in H.
+        destruct (re_compare x1 y1) eqn:E; try(discriminate).
+        destruct IHx1. destruct H0. auto. destruct (re_compare x2 y2); try(discriminate).
+        destruct IHx2. destruct H0; auto.
+      - intros. injection H. intros; subst. simpl.
+        destruct (regex_eq y1 y1) eqn:E.
+        + apply regex_eq_correct in E. apply IHx1 in E. rewrite E.
+          destruct (regex_eq y2 y2) eqn:E1.
+          * apply regex_eq_correct in E1. apply IHx2 in E1. auto.
+          * apply false_not_true in E1. destruct E1. apply regex_eq_correct. auto.
+        + apply false_not_true in E. destruct E. apply regex_eq_correct. auto.
+      - intros. specialize (IHx y). simpl in H. apply IHx in H. subst. auto.
+      - intros. injection H. intros. subst. simpl. apply IHx. auto.
+    Qed.
 
-      Lemma re_compare_eq' : forall x,
-          re_compare x x = Eq.
-      Proof.
-        intros. apply re_compare_eq. auto.
-      Qed.
+    Lemma re_compare_eq' : forall x,
+        re_compare x x = Eq.
+    Proof.
+      intros. apply re_compare_eq. auto.
+    Qed.
 
-      Lemma re_compare_trans : forall c x y z,
-          re_compare x y = c -> re_compare y z = c -> re_compare x z = c.
-      Proof.
-        induction x; destruct y; destruct z; intros; auto;
-          try(simpl in *; subst; discriminate).
-        - simpl in *. eapply compareT_trans; eauto.
-        - simpl in *.
-          destruct(re_compare x1 y1) eqn:E; destruct(re_compare x2 y2) eqn:E0;
-            destruct(re_compare y1 z1) eqn:E1; destruct(re_compare y2 z2) eqn:E2;
-              try(rewrite re_compare_eq in *; subst; repeat rewrite re_compare_eq' in *; auto);
-              try(discriminate);
-              try(specialize (IHx2 y2 z2); apply IHx2; auto);
-              try(rewrite E0; rewrite E1; auto);
-              try(rewrite E1; auto);
-              try(rewrite E; auto);
-              try(specialize (IHx1 y1 z1); rewrite IHx1; [reflexivity|auto|auto]);
-              try(subst; specialize (IHx1 y1 z1); specialize (IHx2 y2 z2);
-                  rewrite IHx1; [reflexivity|auto|auto]); try(discriminate).
-        - simpl in *.
-          destruct(re_compare x1 y1) eqn:E; destruct(re_compare x2 y2) eqn:E0;
-            destruct(re_compare y1 z1) eqn:E1; destruct(re_compare y2 z2) eqn:E2;
-              try(rewrite re_compare_eq in *; subst; repeat rewrite re_compare_eq' in *; auto);
-              try(discriminate);
-              try(specialize (IHx2 y2 z2); apply IHx2; auto);
-              try(rewrite E0; rewrite E1; auto);
-              try(rewrite E1; auto);
-              try(rewrite E; auto);
-              try(specialize (IHx1 y1 z1); rewrite IHx1; [reflexivity|auto|auto]);
-              try(subst; specialize (IHx1 y1 z1); specialize (IHx2 y2 z2);
-                  rewrite IHx1; [reflexivity|auto|auto]); try(discriminate).
-        - simpl in *. eapply IHx; eauto.
-      Qed.
-          
-    End Regexes.
+    Lemma re_compare_trans : forall c x y z,
+        re_compare x y = c -> re_compare y z = c -> re_compare x z = c.
+    Proof.
+      induction x; destruct y; destruct z; intros; auto;
+        try(simpl in *; subst; discriminate).
+      - simpl in *. eapply compareT_trans; eauto.
+      - simpl in *.
+        destruct(re_compare x1 y1) eqn:E; destruct(re_compare x2 y2) eqn:E0;
+          destruct(re_compare y1 z1) eqn:E1; destruct(re_compare y2 z2) eqn:E2;
+            try(rewrite re_compare_eq in *; subst; repeat rewrite re_compare_eq' in *; auto);
+            try(discriminate);
+            try(specialize (IHx2 y2 z2); apply IHx2; auto);
+            try(rewrite E0; rewrite E1; auto);
+            try(rewrite E1; auto);
+            try(rewrite E; auto);
+            try(specialize (IHx1 y1 z1); rewrite IHx1; [reflexivity|auto|auto]);
+            try(subst; specialize (IHx1 y1 z1); specialize (IHx2 y2 z2);
+                rewrite IHx1; [reflexivity|auto|auto]); try(discriminate).
+      - simpl in *.
+        destruct(re_compare x1 y1) eqn:E; destruct(re_compare x2 y2) eqn:E0;
+          destruct(re_compare y1 z1) eqn:E1; destruct(re_compare y2 z2) eqn:E2;
+            try(rewrite re_compare_eq in *; subst; repeat rewrite re_compare_eq' in *; auto);
+            try(discriminate);
+            try(specialize (IHx2 y2 z2); apply IHx2; auto);
+            try(rewrite E0; rewrite E1; auto);
+            try(rewrite E1; auto);
+            try(rewrite E; auto);
+            try(specialize (IHx1 y1 z1); rewrite IHx1; [reflexivity|auto|auto]);
+            try(subst; specialize (IHx1 y1 z1); specialize (IHx2 y2 z2);
+                rewrite IHx1; [reflexivity|auto|auto]); try(discriminate).
+      - simpl in *. eapply IHx; eauto.
+    Qed.
+    
+  End Regexes.
 
-    Module regex_as_UCT <: UsualComparableType.
-      Definition t := regex.
-      Definition compare := re_compare.
-      Definition compare_eq := re_compare_eq.
-      Definition compare_trans := re_compare_trans.
-    End regex_as_UCT.
-      
+  Module regex_as_UCT <: UsualComparableType.
+    Definition t := regex.
+    Definition compare := re_compare.
+    Definition compare_eq := re_compare_eq.
+    Definition compare_trans := re_compare_trans.
+  End regex_as_UCT.
+  
 
-    Module regex_as_UOT <: UsualOrderedType := UOT_from_UCT regex_as_UCT.
+  Module regex_as_UOT <: UsualOrderedType := UOT_from_UCT regex_as_UCT.
 
-    Module reFS := FSetAVL.Make regex_as_UOT.
-    Module reFSF := FSetFacts.Facts reFS.
+  Module reFS := FSetAVL.Make regex_as_UOT.
+  Module reFSF := FSetFacts.Facts reFS.
 
-    Module reFM := FMapAVL.Make regex_as_UOT.
-    Module reFMF := FMapFacts.Facts reFM.
+  Module reFM := FMapAVL.Make regex_as_UOT.
+  Module reFMF := FMapFacts.Facts reFM.
 
-    Module Export MatchSpec.
+  Module Export MatchSpec.
 
-      Inductive exp_match : String -> regex -> Prop :=
-      | MEmpty : exp_match [] EmptyStr
-      | MChar x : exp_match [x] (Char x)
-      | MApp s1 re1 s2 re2
-             (H1 : exp_match s1 re1)
-             (H2 : exp_match s2 re2) :
-          exp_match (s1 ++ s2) (App re1 re2)
-      | MUnionL s1 re1 re2
-                (H1 : exp_match s1 re1) :
-          exp_match s1 (Union re1 re2)
-      | MUnionR re1 s2 re2
-                (H2 : exp_match s2 re2) :
-          exp_match s2 (Union re1 re2)
-      | MStar0 re : exp_match [] (Star re)
-      | MStarApp s1 s2 re
-                 (H1 : exp_match s1 re)
-                 (H2 : exp_match s2 (Star re)) :
-          exp_match (s1 ++ s2) (Star re).
+    Inductive exp_match : String -> regex -> Prop :=
+    | MEmpty : exp_match [] EmptyStr
+    | MChar x : exp_match [x] (Char x)
+    | MApp s1 re1 s2 re2
+           (H1 : exp_match s1 re1)
+           (H2 : exp_match s2 re2) :
+        exp_match (s1 ++ s2) (App re1 re2)
+    | MUnionL s1 re1 re2
+              (H1 : exp_match s1 re1) :
+        exp_match s1 (Union re1 re2)
+    | MUnionR re1 s2 re2
+              (H2 : exp_match s2 re2) :
+        exp_match s2 (Union re1 re2)
+    | MStar0 re : exp_match [] (Star re)
+    | MStarApp s1 s2 re
+               (H1 : exp_match s1 re)
+               (H2 : exp_match s2 (Star re)) :
+        exp_match (s1 ++ s2) (Star re).
 
-      Definition re_equiv (e1 e2 : regex) : Prop :=
-        forall z, exp_match z e1 <-> exp_match z e2.
+    Definition re_equiv (e1 e2 : regex) : Prop :=
+      forall z, exp_match z e1 <-> exp_match z e2.
 
-    End MatchSpec.
+  End MatchSpec.
 
-    Module Export MatchSpecLemmas.
-      
-      Theorem nullable_bridge : forall(r : regex),
-        true = nullable r <-> exp_match [] r.
-      Proof.
-        intros r. split; intros H.
-        - induction r; try(simpl in H; discriminate).
-          + apply MEmpty.
-          + simpl in H. destruct (nullable r1); destruct (nullable r2); try(simpl in H; discriminate).
-            rewrite <- nil_left with (s := []). apply MApp.
-            * apply IHr1. reflexivity.
-            * apply IHr2. reflexivity.
-          + simpl in H.  destruct (nullable r1); destruct (nullable r2).
-            * apply MUnionL. apply IHr1. reflexivity.
-            * apply MUnionL. apply IHr1. reflexivity.
-            * apply MUnionR. apply IHr2. reflexivity.
-            * simpl in H. discriminate.
-          + apply MStar0.
-        - induction r.
-          + inversion H.
-          + simpl. reflexivity.
-          + inversion H.
-          + simpl. inversion H. apply empty_app in H1. destruct H1.
-            rewrite H1 in H3. rewrite H5 in H4.
-            apply IHr1 in H3. apply IHr2 in H4.
-            rewrite <- H3. rewrite <- H4. simpl. reflexivity.
-          + simpl. inversion H.
-            * apply IHr1 in H2. rewrite <- H2. destruct (nullable r2); simpl; reflexivity.
-            * apply IHr2 in H1. rewrite <- H1. destruct (nullable r1); simpl; reflexivity.
-          + simpl. reflexivity.
-      Qed.
+  Module Export MatchSpecLemmas.
+    
+    Theorem nullable_bridge : forall(r : regex),
+      true = nullable r <-> exp_match [] r.
+    Proof.
+      intros r. split; intros H.
+      - induction r; try(simpl in H; discriminate).
+        + apply MEmpty.
+        + simpl in H. destruct (nullable r1); destruct (nullable r2); try(simpl in H; discriminate).
+          rewrite <- nil_left with (s := []). apply MApp.
+          * apply IHr1. reflexivity.
+          * apply IHr2. reflexivity.
+        + simpl in H.  destruct (nullable r1); destruct (nullable r2).
+          * apply MUnionL. apply IHr1. reflexivity.
+          * apply MUnionL. apply IHr1. reflexivity.
+          * apply MUnionR. apply IHr2. reflexivity.
+          * simpl in H. discriminate.
+        + apply MStar0.
+      - induction r.
+        + inversion H.
+        + simpl. reflexivity.
+        + inversion H.
+        + simpl. inversion H. apply empty_app in H1. destruct H1.
+          rewrite H1 in H3. rewrite H5 in H4.
+          apply IHr1 in H3. apply IHr2 in H4.
+          rewrite <- H3. rewrite <- H4. simpl. reflexivity.
+        + simpl. inversion H.
+          * apply IHr1 in H2. rewrite <- H2. destruct (nullable r2); simpl; reflexivity.
+          * apply IHr2 in H1. rewrite <- H1. destruct (nullable r1); simpl; reflexivity.
+        + simpl. reflexivity.
+    Qed.
 
-      Theorem nullable_bridge' : forall(r : regex),
-          nullable r = true <-> exp_match [] r.
-      Proof.
-        split; intros.
-        - symmetry in H. apply nullable_bridge; auto.
-        - symmetry. apply nullable_bridge; auto.
-      Qed.
+    Theorem nullable_bridge' : forall(r : regex),
+        nullable r = true <-> exp_match [] r.
+    Proof.
+      split; intros.
+      - symmetry in H. apply nullable_bridge; auto.
+      - symmetry. apply nullable_bridge; auto.
+    Qed.
 
-      
-      
+    
+    
 
-      (* star_concat upto concat_star necessary for hard star case of der_match *)
-      Lemma star_concat :
-        forall s r',
-          exp_match s (Star r')
-          -> (exists xss : list (list Sigma),
-                s = concat xss
-                /\ (forall xs,
-                      In xs xss
-                      -> exp_match xs r')).
-      Proof.
-        intros s r' hm.
-        remember (Star r') as r. generalize dependent r'.
-        induction hm; intros r' heq; inv heq.
-        - exists []; split; auto.
-          intros xs hi; inv hi.
-        - destruct (IHhm2 r') as (xss' & heq & hall); subst; auto.
-          exists (s1 :: xss'); split; auto.
-          intros xs hi.
-          destruct hi as [hh| ht]; subst; auto.
-      Qed.
+    (* star_concat upto concat_star necessary for hard star case of der_match *)
+    Lemma star_concat :
+      forall s r',
+        exp_match s (Star r')
+        -> (exists xss : list (list Sigma),
+              s = concat xss
+              /\ (forall xs,
+                    In xs xss
+                    -> exp_match xs r')).
+    Proof.
+      intros s r' hm.
+      remember (Star r') as r. generalize dependent r'.
+      induction hm; intros r' heq; inv heq.
+      - exists []; split; auto.
+        intros xs hi; inv hi.
+      - destruct (IHhm2 r') as (xss' & heq & hall); subst; auto.
+        exists (s1 :: xss'); split; auto.
+        intros xs hi.
+        destruct hi as [hh| ht]; subst; auto.
+    Qed.
 
-      Lemma star_concat_no_empt : forall(s : String) (r' : regex),
-          s <> []
-          -> exp_match s (Star r')
-          -> (exists xss : list (list Sigma),
-                s = concat xss
-                /\ (forall xs,
-                      In xs xss
-                      -> exp_match xs r' /\ xs <> [])).
-      Proof.
-        intros s r' Hempty Hstar. apply star_concat in Hstar.
-        destruct Hstar as (yss & heq & hall).
-        exists(rm_empty yss). split.
-        - rewrite rm_empty_mute. apply heq.
-        - intros xs H. split.
-          + apply hall.  apply filtered_subset in H. apply H.
-          + apply rm_empty_no_empty in H. apply H.
-      Qed.
+    Lemma star_concat_no_empt : forall(s : String) (r' : regex),
+        s <> []
+        -> exp_match s (Star r')
+        -> (exists xss : list (list Sigma),
+              s = concat xss
+              /\ (forall xs,
+                    In xs xss
+                    -> exp_match xs r' /\ xs <> [])).
+    Proof.
+      intros s r' Hempty Hstar. apply star_concat in Hstar.
+      destruct Hstar as (yss & heq & hall).
+      exists(rm_empty yss). split.
+      - rewrite rm_empty_mute. apply heq.
+      - intros xs H. split.
+        + apply hall.  apply filtered_subset in H. apply H.
+        + apply rm_empty_no_empty in H. apply H.
+    Qed.
 
-      Lemma concat_star : forall(xss : list String) (r : regex),
-          (forall xs : list Sigma, In xs xss -> exp_match xs r) -> exp_match (concat xss) (Star r).
-      Proof.
-        intros xss r H. induction xss.
-        - simpl. apply MStar0.
-        - replace (concat (a :: xss)) with (a ++ (concat xss)).
+    Lemma concat_star : forall(xss : list String) (r : regex),
+        (forall xs : list Sigma, In xs xss -> exp_match xs r) -> exp_match (concat xss) (Star r).
+    Proof.
+      intros xss r H. induction xss.
+      - simpl. apply MStar0.
+      - replace (concat (a :: xss)) with (a ++ (concat xss)).
+        + apply MStarApp.
+          * apply H. simpl. left. reflexivity.
+          * apply IHxss. intros xs H1. apply H. simpl. right. apply H1.
+        + simpl. reflexivity.
+    Qed.
+
+    Theorem der_match : forall(a : Sigma) (s : String) (r : regex),
+        exp_match (a::s) r <-> exp_match s (derivative a r).
+    Proof.
+      intros a s r.
+      split.
+      {
+        generalize dependent s. induction r; intros s H.
+        - inv H.
+        - inv H.
+        - destruct s.
+          + simpl. destruct (Sigma_dec t a).
+            * apply MEmpty.
+            * inv H. contradiction.
+          + inv H.
+        - simpl. destruct(nullable r1) eqn:E.
+          + inv H. destruct s1.
+            * apply MUnionR. apply IHr2. rewrite <- H1. simpl. apply H4.
+            * apply MUnionL. simpl in H1. injection H1. intros Happ Hchar.
+              rewrite <- Happ. rewrite Hchar in H3. apply IHr1 in H3.
+              apply MApp.
+              -- apply H3.
+              -- apply H4.
+          + inv H. destruct s1.
+            * apply nullable_bridge in H3. rewrite E in H3. discriminate.
+            * simpl in H1. injection H1. intros Happ Hchar.
+              rewrite <- Happ. rewrite Hchar in H3. apply IHr1 in H3.
+              apply MApp.
+              -- apply H3.
+              -- apply H4.
+        - simpl. inv H.
+          + apply IHr1 in H2. apply MUnionL. apply H2.
+          + apply IHr2 in H1. apply MUnionR. apply H1.
+        (* hard_star: This case was the hard one *)
+        - apply star_concat_no_empt in H. destruct H as (xss & heq & hall).
+          + assert (H : exists(s1 : String) (yss : list String),
+                       ((a :: s1) :: yss) = xss).
+            {
+              destruct xss.
+              - simpl in heq. discriminate.
+              - simpl in heq. destruct l eqn:E.
+                + apply hall in E.
+                  * contradiction.
+                  * rewrite E. simpl. left. reflexivity.
+                + exists(l0). exists(xss). simpl in heq.
+                  injection heq. intros I1 I2. rewrite I2. reflexivity.
+            }
+            destruct H as [s1]. destruct H as [yss].
+            rewrite <- H in hall.
+            assert (A : In (a :: s1) ((a :: s1) :: yss)).
+            { simpl. left. reflexivity. }
+            simpl. replace s with (s1 ++ (concat yss)).
+            * apply MApp.
+              -- apply IHr. apply hall in A. destruct A. apply H0.
+              -- rewrite H in hall.
+                 assert (A1 : forall xs : list Sigma, In xs xss -> exp_match xs r).
+                 { intros xs. intros HA1. apply hall in HA1. destruct HA1. apply H0. }
+                 apply concat_star. intros xs H1. apply A1.
+                 rewrite <- H. simpl. right. apply H1.
+            * assert (A1 : concat ((a :: s1) :: yss) = concat xss).
+              { rewrite H. reflexivity. }
+              assert (A2 : concat ((a :: s1) :: yss) = a :: (s1 ++ (concat yss))).
+              { simpl. reflexivity. }
+              rewrite <- A1 in heq. rewrite A2 in heq. injection heq.
+              intros I. symmetry. apply I.
+          + unfold not. intros C. discriminate.
+      }
+      {
+        generalize dependent s. induction r; intros s H.
+        - inv H.
+        - inv H.
+        - simpl in H. destruct (Sigma_dec t a); inv H. apply MChar.
+        - simpl in H. destruct (nullable r1) eqn:E.
+          + inv H.
+            * inv H2. replace (a :: s1 ++ s2) with ((a :: s1) ++ s2).
+              apply MApp.
+              -- apply IHr1. apply H3.
+              -- apply H4.
+              -- reflexivity.
+            * symmetry in E. apply nullable_bridge in E. rewrite <- nil_left with (s := (a :: s)).
+              apply MApp.
+              -- apply E.
+              -- apply IHr2. apply H1.
+          + inv H.
+            * replace (a :: s1 ++ s2) with ((a :: s1) ++ s2).
+              apply MApp.
+              -- apply IHr1. apply H3.
+              -- apply H4.
+              -- reflexivity.
+        - inv H.
+          + apply MUnionL. apply IHr1. apply H2.
+          + apply MUnionR. apply IHr2. apply H1.
+        - simpl in H. inv H. replace (a :: s1 ++ s2) with ((a :: s1) ++ s2).
           + apply MStarApp.
-            * apply H. simpl. left. reflexivity.
-            * apply IHxss. intros xs H1. apply H. simpl. right. apply H1.
-          + simpl. reflexivity.
-      Qed.
+            * apply IHr. apply H3.
+            * apply H4.
+          + reflexivity.
+      }
+    Qed.
 
-      Theorem der_match : forall(a : Sigma) (s : String) (r : regex),
-          exp_match (a::s) r <-> exp_match s (derivative a r).
-      Proof.
-        intros a s r.
-        split.
-        {
-          generalize dependent s. induction r; intros s H.
-          - inv H.
-          - inv H.
-          - destruct s.
-            + simpl. destruct (Sigma_dec t a).
-              * apply MEmpty.
-              * inv H. contradiction.
-            + inv H.
-          - simpl. destruct(nullable r1) eqn:E.
-            + inv H. destruct s1.
-              * apply MUnionR. apply IHr2. rewrite <- H1. simpl. apply H4.
-              * apply MUnionL. simpl in H1. injection H1. intros Happ Hchar.
-                rewrite <- Happ. rewrite Hchar in H3. apply IHr1 in H3.
-                apply MApp.
-                -- apply H3.
-                -- apply H4.
-            + inv H. destruct s1.
-              * apply nullable_bridge in H3. rewrite E in H3. discriminate.
-              * simpl in H1. injection H1. intros Happ Hchar.
-                rewrite <- Happ. rewrite Hchar in H3. apply IHr1 in H3.
-                apply MApp.
-                -- apply H3.
-                -- apply H4.
-          - simpl. inv H.
-            + apply IHr1 in H2. apply MUnionL. apply H2.
-            + apply IHr2 in H1. apply MUnionR. apply H1.
-          (* hard_star: This case was the hard one *)
-          - apply star_concat_no_empt in H. destruct H as (xss & heq & hall).
-            + assert (H : exists(s1 : String) (yss : list String),
-                         ((a :: s1) :: yss) = xss).
-              {
-                destruct xss.
-                - simpl in heq. discriminate.
-                - simpl in heq. destruct l eqn:E.
-                  + apply hall in E.
-                    * contradiction.
-                    * rewrite E. simpl. left. reflexivity.
-                  + exists(l0). exists(xss). simpl in heq.
-                    injection heq. intros I1 I2. rewrite I2. reflexivity.
-              }
-              destruct H as [s1]. destruct H as [yss].
-              rewrite <- H in hall.
-              assert (A : In (a :: s1) ((a :: s1) :: yss)).
-              { simpl. left. reflexivity. }
-              simpl. replace s with (s1 ++ (concat yss)).
-              * apply MApp.
-                -- apply IHr. apply hall in A. destruct A. apply H0.
-                -- rewrite H in hall.
-                   assert (A1 : forall xs : list Sigma, In xs xss -> exp_match xs r).
-                   { intros xs. intros HA1. apply hall in HA1. destruct HA1. apply H0. }
-                   apply concat_star. intros xs H1. apply A1.
-                   rewrite <- H. simpl. right. apply H1.
-              * assert (A1 : concat ((a :: s1) :: yss) = concat xss).
-                { rewrite H. reflexivity. }
-                assert (A2 : concat ((a :: s1) :: yss) = a :: (s1 ++ (concat yss))).
-                { simpl. reflexivity. }
-                rewrite <- A1 in heq. rewrite A2 in heq. injection heq.
-                intros I. symmetry. apply I.
-            + unfold not. intros C. discriminate.
-        }
-        {
-          generalize dependent s. induction r; intros s H.
-          - inv H.
-          - inv H.
-          - simpl in H. destruct (Sigma_dec t a); inv H. apply MChar.
-          - simpl in H. destruct (nullable r1) eqn:E.
-            + inv H.
-              * inv H2. replace (a :: s1 ++ s2) with ((a :: s1) ++ s2).
-                apply MApp.
-                -- apply IHr1. apply H3.
-                -- apply H4.
-                -- reflexivity.
-              * symmetry in E. apply nullable_bridge in E. rewrite <- nil_left with (s := (a :: s)).
-                apply MApp.
-                -- apply E.
-                -- apply IHr2. apply H1.
-            + inv H.
-              * replace (a :: s1 ++ s2) with ((a :: s1) ++ s2).
-                apply MApp.
-                -- apply IHr1. apply H3.
-                -- apply H4.
-                -- reflexivity.
-          - inv H.
-            + apply MUnionL. apply IHr1. apply H2.
-            + apply MUnionR. apply IHr2. apply H1.
-          - simpl in H. inv H. replace (a :: s1 ++ s2) with ((a :: s1) ++ s2).
-            + apply MStarApp.
-              * apply IHr. apply H3.
-              * apply H4.
-            + reflexivity.
-        }
-      Qed.
+    Lemma derivative_list_cons : forall bs b e,
+        derivative_list (b :: bs) e = derivative_list bs (derivative b e).
+    Proof.
+      auto.
+    Qed.
 
-      Lemma derivative_list_cons : forall bs b e,
-          derivative_list (b :: bs) e = derivative_list bs (derivative b e).
-      Proof.
-        auto.
-      Qed.
-
-      Lemma derivative_list_str : forall bs e,
-          exp_match [] (derivative_list bs e) <-> exp_match bs e.
-      Proof.
-        induction bs; intros; auto.
-        - simpl. split; auto.
-        - simpl. rewrite IHbs. split; apply der_match.
-      Qed.
-      
-    End MatchSpecLemmas.
-
-    Module Notations.
-      
-      Notation "e1 = e2 " := (regex_eq e1 e2) (at level 70).
-      Notation "a ∂ r" := (derivative a r) (at level 75, right associativity).
-      Notation ε := EmptyStr.
-      Notation "e1 @ e2" := (App e1 e2) (at level 75).
-      Notation "e1 # e2" := (Union e1 e2) (at level 75).
-
-    End Notations.
-
+    Lemma derivative_list_str : forall bs e,
+        exp_match [] (derivative_list bs e) <-> exp_match bs e.
+    Proof.
+      induction bs; intros; auto.
+      - simpl. split; auto.
+      - simpl. rewrite IHbs. split; apply der_match.
+    Qed.
     
+  End MatchSpecLemmas.
 
-    Module Helpers.
-      
-      Definition Plus (r : regex) : regex := App r (Star r).
-
-      Fixpoint IterUnion (rs : list regex) :=
-        match rs with
-        | [] => EmptySet
-        | [e] => e
-        | h::t => Union h (IterUnion t)
-        end.
-
-      Fixpoint IterApp (rs : list regex) :=
-        match rs with
-        | [] => EmptyStr
-        | [e] => e
-        | h::t => App h (IterApp t)
-        end.
-
-      (* r? *)
-      Definition Optional (r : regex) := Union EmptyStr r.
-
-      Definition REString (z : String) := IterApp (map Char z).
-
-    End Helpers.
+  Module Notations.
     
+    Notation "e1 = e2 " := (regex_eq e1 e2) (at level 70).
+    Notation "a ∂ r" := (derivative a r) (at level 75, right associativity).
+    Notation ε := EmptyStr.
+    Notation "e1 @ e2" := (App e1 e2) (at level 75).
+    Notation "e1 # e2" := (Union e1 e2) (at level 75).
+
+  End Notations.
+
+  
+
+  Module Helpers.
+    
+    Definition Plus (r : regex) : regex := App r (Star r).
+
+    Fixpoint IterUnion (rs : list regex) :=
+      match rs with
+      | [] => EmptySet
+      | [e] => e
+      | h::t => Union h (IterUnion t)
+      end.
+
+    Fixpoint IterApp (rs : list regex) :=
+      match rs with
+      | [] => EmptyStr
+      | [e] => e
+      | h::t => App h (IterApp t)
+      end.
+
+    (* r? *)
+    Definition Optional (r : regex) := Union EmptyStr r.
+
+    Definition REString (z : String) := IterApp (map Char z).
+
+  End Helpers.
+  
 End DefsFn.
 
 
